chore: reorganisation of `List` API (#4469)
This PR neither adds nor removes material, but improves the organization
of `Init/Data/List/*`.

These files are essentially completely re-ordered, to ensure that
material is developed in a consistent order between `List.Basic`,
`List.Impl`, `List.BasicAux`, and `List.Lemmas`.

Everything is organised in subsections, and I've added some module docs.

src/Init/Data/List/Lemmas.lean
@@ -12,34 +12,108 @@ import Init.PropLemmas
 import Init.Control.Lawful.Basic
 import Init.Hints
 
+/-! # Theorems about `List` operations.
+
+For each `List` operation, we would like theorems describing the following, when relevant:
+* if it is a "convenience" function, a `@[simp]` lemma reducing it to more basic operations
+  (e.g. `List.partition_eq_filter_filter`), and otherwise:
+* any special cases of equational lemmas that require additional hypotheses
+* lemmas for special cases of the arguments (e.g. `List.map_id`)
+* the length of the result `(f L).length`
+* the `i`-th element, described via `(f L)[i]` and/or `(f L)[i]?` (these should typically be `@[simp]`)
+* consequences for `f L` of the fact `x ∈ L` or `x ∉ L`
+* conditions characterising `x ∈ f L` (often but not always `@[simp]`)
+* injectivity statements, or congruence statements of the form `p L M → f L = f M`.
+* conditions characterising the result, i.e. of the form `f L = M ↔ p M` for some predicate `p`,
+  along with special cases of `M` (e.g. `List.append_eq_nil : L ++ M = [] ↔ L = [] ∧ M = []`)
+* negative characterisations are also useful, e.g. `List.cons_ne_nil`
+* interactions with all previously described `List` operations where possible
+  (some of these should be `@[simp]`, particularly if the result can be described by a single operation)
+* characterising `(∀ (i) (_ : i ∈ f L), P i)`, for some predicate `P`
+
+Of course for any individual operation, not all of these will be relevant or helpful, so some judgement is required.
+
+-/
 namespace List
 
 open Nat
 
-attribute [simp] concat_eq_append append_assoc
+-- We may want to replace these `simp` attributes with explicit equational lemmas,
+-- as we already have for all the non-monadic functions.
+attribute [simp] mapA forA filterAuxM firstM anyM allM findM? findSomeM?
 
-@[simp] theorem get?_nil : @get? α [] n = none := rfl
-@[simp] theorem get?_cons_zero : @get? α (a::l) 0 = some a := rfl
-@[simp] theorem get?_cons_succ : @get? α (a::l) (n+1) = get? l n := rfl
+-- Previously `range.loop`, `mapM.loop`, `filterMapM.loop`, `forIn.loop`, `forIn'.loop`
+-- had attribute `@[simp]`.
+-- We don't currently provide simp lemmas,
+-- as this is an internal implementation and they don't seem to be needed.
+
+/-! ### cons -/
+
+theorem cons_ne_nil (a : α) (l : List α) : a :: l ≠ [] := nofun
+
+@[simp]
+theorem cons_ne_self (a : α) (l : List α) : a :: l ≠ l := mt (congrArg length) (Nat.succ_ne_self _)
+
+theorem head_eq_of_cons_eq (H : h₁ :: t₁ = h₂ :: t₂) : h₁ = h₂ := (cons.inj H).1
+
+theorem tail_eq_of_cons_eq (H : h₁ :: t₁ = h₂ :: t₂) : t₁ = t₂ := (cons.inj H).2
+
+theorem cons_inj (a : α) {l l' : List α} : a :: l = a :: l' ↔ l = l' :=
+  ⟨tail_eq_of_cons_eq, congrArg _⟩
+
+theorem cons_eq_cons {a b : α} {l l' : List α} : a :: l = b :: l' ↔ a = b ∧ l = l' :=
+  List.cons.injEq .. ▸ .rfl
+
+theorem exists_cons_of_ne_nil : ∀ {l : List α}, l ≠ [] → ∃ b L, l = b :: L
+  | c :: l', _ => ⟨c, l', rfl⟩
+
+/-! ### length -/
+
+theorem eq_nil_of_length_eq_zero (_ : length l = 0) : l = [] := match l with | [] => rfl
+
+theorem ne_nil_of_length_eq_succ (_ : length l = succ n) : l ≠ [] := fun _ => nomatch l
+
+@[simp] theorem length_eq_zero : length l = 0 ↔ l = [] :=
+  ⟨eq_nil_of_length_eq_zero, fun h => h ▸ rfl⟩
+
+theorem length_pos_of_mem {a : α} : ∀ {l : List α}, a ∈ l → 0 < length l
+  | _::_, _ => Nat.zero_lt_succ _
+
+theorem exists_mem_of_length_pos : ∀ {l : List α}, 0 < length l → ∃ a, a ∈ l
+  | _::_, _ => ⟨_, .head ..⟩
+
+theorem length_pos_iff_exists_mem {l : List α} : 0 < length l ↔ ∃ a, a ∈ l :=
+  ⟨exists_mem_of_length_pos, fun ⟨_, h⟩ => length_pos_of_mem h⟩
+
+theorem exists_cons_of_length_pos : ∀ {l : List α}, 0 < l.length → ∃ h t, l = h :: t
+  | _::_, _ => ⟨_, _, rfl⟩
+
+theorem length_pos_iff_exists_cons :
+    ∀ {l : List α}, 0 < l.length ↔ ∃ h t, l = h :: t :=
+  ⟨exists_cons_of_length_pos, fun ⟨_, _, eq⟩ => eq ▸ Nat.succ_pos _⟩
+
+theorem exists_cons_of_length_succ :
+    ∀ {l : List α}, l.length = n + 1 → ∃ h t, l = h :: t
+  | _::_, _ => ⟨_, _, rfl⟩
+
+theorem length_pos {l : List α} : 0 < length l ↔ l ≠ [] :=
+  Nat.pos_iff_ne_zero.trans (not_congr length_eq_zero)
+
+theorem exists_mem_of_ne_nil (l : List α) (h : l ≠ []) : ∃ x, x ∈ l :=
+  exists_mem_of_length_pos (length_pos.2 h)
+
+theorem length_eq_one {l : List α} : length l = 1 ↔ ∃ a, l = [a] :=
+  ⟨fun h => match l, h with | [_], _ => ⟨_, rfl⟩, fun ⟨_, h⟩ => by simp [h]⟩
+
+/-! ### L[i] and L[i]? -/
+
 @[simp] theorem get_cons_zero : get (a::l) (0 : Fin (l.length + 1)) = a := rfl
-@[simp] theorem head?_nil : @head? α [] = none := rfl
-@[simp] theorem head?_cons : @head? α (a::l) = some a := rfl
-@[simp 1100] theorem headD_nil : @headD α [] d = d := rfl
-@[simp 1100] theorem headD_cons : @headD α (a::l) d = a := rfl
-@[simp] theorem head_cons : @head α (a::l) h = a := rfl
-@[simp] theorem tail?_nil : @tail? α [] = none := rfl
-@[simp] theorem tail?_cons : @tail? α (a::l) = some l := rfl
-@[simp] theorem tail!_cons : @tail! α (a::l) = l := rfl
-@[simp 1100] theorem tailD_nil : @tailD α [] l' = l' := rfl
-@[simp 1100] theorem tailD_cons : @tailD α (a::l) l' = l := rfl
-@[simp] theorem any_nil : [].any f = false := rfl
-@[simp] theorem any_cons : (a::l).any f = (f a || l.any f) := rfl
-@[simp] theorem all_nil : [].all f = true := rfl
-@[simp] theorem all_cons : (a::l).all f = (f a && l.all f) := rfl
-@[simp] theorem or_nil : [].or = false := rfl
-@[simp] theorem or_cons : (a::l).or = (a || l.or) := rfl
-@[simp] theorem and_nil : [].and = true := rfl
-@[simp] theorem and_cons : (a::l).and = (a && l.and) := rfl
+
+@[simp] theorem get_cons_succ {as : List α} {h : i + 1 < (a :: as).length} :
+  (a :: as).get ⟨i+1, h⟩ = as.get ⟨i, Nat.lt_of_succ_lt_succ h⟩ := rfl
+
+@[simp] theorem get_cons_succ' {as : List α} {i : Fin as.length} :
+  (a :: as).get i.succ = as.get i := rfl
 
 theorem get?_len_le : ∀ {l : List α} {n}, length l ≤ n → l.get? n = none
   | [], _, _ => rfl
@@ -99,14 +173,110 @@ theorem getElem?_eq_some {l : List α} : l[n]? = some a ↔ ∃ h : n < l.length
   · rw [getElem!_pos, getElem!_pos] <;> simp_all [Nat.succ_lt_succ_iff]
   · rw [getElem!_neg, getElem!_neg] <;> simp_all [Nat.succ_lt_succ_iff]
 
-/-! ### length -/
+@[simp] theorem get_cons_cons_one : (a₁ :: a₂ :: as).get (1 : Fin (as.length + 2)) = a₂ := rfl
 
-theorem eq_nil_of_length_eq_zero (_ : length l = 0) : l = [] := match l with | [] => rfl
+theorem get!_len_le [Inhabited α] : ∀ {l : List α} {n}, length l ≤ n → l.get! n = (default : α)
+  | [], _, _ => rfl
+  | _ :: l, _+1, h => get!_len_le (l := l) <| Nat.le_of_succ_le_succ h
 
-theorem ne_nil_of_length_eq_succ (_ : length l = succ n) : l ≠ [] := fun _ => nomatch l
+theorem get?_zero (l : List α) : l.get? 0 = l.head? := by cases l <;> rfl
 
-@[simp] theorem length_eq_zero : length l = 0 ↔ l = [] :=
-  ⟨eq_nil_of_length_eq_zero, fun h => h ▸ rfl⟩
+/--
+If one has `l[i]` in an expression and `h : l = l'`,
+`rw [h]` will give a "motive it not type correct" error, as it cannot rewrite the
+implicit `i < l.length` to `i < l'.length` directly. The theorem `getElem_of_eq` can be used to make
+such a rewrite, with `rw [getElem_of_eq h]`.
+-/
+theorem getElem_of_eq {l l' : List α} (h : l = l') {i : Nat} (w : i < l.length) :
+    l[i] = l'[i]'(h ▸ w) := by cases h; rfl
+
+/--
+If one has `l.get i` in an expression (with `i : Fin l.length`) and `h : l = l'`,
+`rw [h]` will give a "motive it not type correct" error, as it cannot rewrite the
+`i : Fin l.length` to `Fin l'.length` directly. The theorem `get_of_eq` can be used to make
+such a rewrite, with `rw [get_of_eq h]`.
+-/
+theorem get_of_eq {l l' : List α} (h : l = l') (i : Fin l.length) :
+    get l i = get l' ⟨i, h ▸ i.2⟩ := by cases h; rfl
+
+@[simp] theorem getElem_singleton (a : α) (h : i < 1) : [a][i] = a :=
+  match i, h with
+  | 0, _ => rfl
+
+@[deprecated getElem_singleton (since := "2024-06-12")]
+theorem get_singleton (a : α) (n : Fin 1) : get [a] n = a := by simp
+
+theorem getElem_zero {l : List α} (h : 0 < l.length) : l[0] = l.head (length_pos.mp h) :=
+  match l, h with
+  | _ :: _, _ => rfl
+
+theorem get_mk_zero : ∀ {l : List α} (h : 0 < l.length), l.get ⟨0, h⟩ = l.head (length_pos.mp h)
+  | _::_, _ => rfl
+
+theorem getElem!_of_getElem? [Inhabited α] : ∀ {l : List α} {n : Nat}, l[n]? = some a → l[n]! = a
+  | _a::_, 0, _ => by
+    rw [getElem!_pos] <;> simp_all
+  | _::l, _+1, e => by
+    simp at e
+    simp_all [getElem!_of_getElem? (l := l) e]
+
+theorem get!_of_get? [Inhabited α] : ∀ {l : List α} {n}, get? l n = some a → get! l n = a
+  | _a::_, 0, rfl => rfl
+  | _::l, _+1, e => get!_of_get? (l := l) e
+
+@[simp] theorem get!_eq_getD [Inhabited α] : ∀ (l : List α) n, l.get! n = l.getD n default
+  | [], _      => rfl
+  | _a::_, 0   => rfl
+  | _a::l, n+1 => get!_eq_getD l n
+
+@[ext] theorem ext_getElem? {l₁ l₂ : List α} (h : ∀ n : Nat, l₁[n]? = l₂[n]?) : l₁ = l₂ :=
+  ext_get? fun n => by simp_all
+
+theorem ext_getElem {l₁ l₂ : List α} (hl : length l₁ = length l₂)
+    (h : ∀ (n : Nat) (h₁ : n < l₁.length) (h₂ : n < l₂.length), l₁[n]'h₁ = l₂[n]'h₂) : l₁ = l₂ :=
+  ext_getElem? fun n =>
+    if h₁ : n < length l₁ then by
+      simp_all [getElem?_eq_getElem]
+    else by
+      have h₁ := Nat.le_of_not_lt h₁
+      rw [getElem?_len_le h₁, getElem?_len_le]; rwa [← hl]
+
+theorem ext_get {l₁ l₂ : List α} (hl : length l₁ = length l₂)
+    (h : ∀ n h₁ h₂, get l₁ ⟨n, h₁⟩ = get l₂ ⟨n, h₂⟩) : l₁ = l₂ :=
+  ext_getElem hl (by simp_all)
+
+@[simp] theorem getElem?_concat_length : ∀ (l : List α) (a : α), (l ++ [a])[l.length]? = some a
+  | [], a => rfl
+  | b :: l, a => by rw [cons_append, length_cons]; simp [getElem?_concat_length]
+
+@[deprecated getElem?_concat_length (since := "2024-06-12")]
+theorem get?_concat_length (l : List α) (a : α) : (l ++ [a]).get? l.length = some a := by simp
+
+/-! ### concat -/
+
+-- As `List.concat` is defined in `Init.Prelude`, we write the basic simplification lemmas here.
+theorem concat_nil (a : α) : concat [] a = [a] :=
+  rfl
+theorem concat_cons (a b : α) (l : List α) : concat (a :: l) b = a :: concat l b :=
+  rfl
+
+theorem init_eq_of_concat_eq {a : α} {l₁ l₂ : List α} : concat l₁ a = concat l₂ a → l₁ = l₂ := by
+  simp
+
+theorem last_eq_of_concat_eq {a b : α} {l : List α} : concat l a = concat l b → a = b := by
+  simp
+
+theorem concat_ne_nil (a : α) (l : List α) : concat l a ≠ [] := by cases l <;> simp
+
+theorem concat_append (a : α) (l₁ l₂ : List α) : concat l₁ a ++ l₂ = l₁ ++ a :: l₂ := by simp
+
+theorem append_concat (a : α) (l₁ l₂ : List α) : l₁ ++ concat l₂ a = concat (l₁ ++ l₂) a := by simp
+
+theorem eq_nil_or_concat : ∀ l : List α, l = [] ∨ ∃ L b, l = L ++ [b]
+  | [] => .inl rfl
+  | a::l => match l, eq_nil_or_concat l with
+    | _, .inl rfl => .inr ⟨[], a, rfl⟩
+    | _, .inr ⟨L, b, rfl⟩ => .inr ⟨a::L, b, rfl⟩
 
 /-! ### mem -/
 
@@ -123,124 +293,57 @@ theorem mem_cons_of_mem (y : α) {a : α} {l : List α} : a ∈ l → a ∈ y ::
 theorem eq_nil_iff_forall_not_mem {l : List α} : l = [] ↔ ∀ a, a ∉ l := by
   cases l <;> simp [-not_or]
 
-/-! ### append -/
+theorem eq_of_mem_singleton : a ∈ [b] → a = b
+  | .head .. => rfl
 
-@[simp 1100] theorem singleton_append : [x] ++ l = x :: l := rfl
-
-theorem append_inj :
-    ∀ {s₁ s₂ t₁ t₂ : List α}, s₁ ++ t₁ = s₂ ++ t₂ → length s₁ = length s₂ → s₁ = s₂ ∧ t₁ = t₂
-  | [], [], t₁, t₂, h, _ => ⟨rfl, h⟩
-  | a :: s₁, b :: s₂, t₁, t₂, h, hl => by
-    simp [append_inj (cons.inj h).2 (Nat.succ.inj hl)] at h ⊢; exact h
-
-theorem append_inj_right (h : s₁ ++ t₁ = s₂ ++ t₂) (hl : length s₁ = length s₂) : t₁ = t₂ :=
-  (append_inj h hl).right
-
-theorem append_inj_left (h : s₁ ++ t₁ = s₂ ++ t₂) (hl : length s₁ = length s₂) : s₁ = s₂ :=
-  (append_inj h hl).left
-
-theorem append_inj' (h : s₁ ++ t₁ = s₂ ++ t₂) (hl : length t₁ = length t₂) : s₁ = s₂ ∧ t₁ = t₂ :=
-  append_inj h <| @Nat.add_right_cancel _ (length t₁) _ <| by
-  let hap := congrArg length h; simp only [length_append, ← hl] at hap; exact hap
-
-theorem append_inj_right' (h : s₁ ++ t₁ = s₂ ++ t₂) (hl : length t₁ = length t₂) : t₁ = t₂ :=
-  (append_inj' h hl).right
-
-theorem append_inj_left' (h : s₁ ++ t₁ = s₂ ++ t₂) (hl : length t₁ = length t₂) : s₁ = s₂ :=
-  (append_inj' h hl).left
-
-theorem append_right_inj {t₁ t₂ : List α} (s) : s ++ t₁ = s ++ t₂ ↔ t₁ = t₂ :=
-  ⟨fun h => append_inj_right h rfl, congrArg _⟩
-
-theorem append_left_inj {s₁ s₂ : List α} (t) : s₁ ++ t = s₂ ++ t ↔ s₁ = s₂ :=
-  ⟨fun h => append_inj_left' h rfl, congrArg (· ++ _)⟩
-
-@[simp] theorem append_eq_nil : p ++ q = [] ↔ p = [] ∧ q = [] := by
-  cases p <;> simp
-
-theorem getElem_append : ∀ {l₁ l₂ : List α} (n : Nat) (h : n < l₁.length),
-    (l₁ ++ l₂)[n]'(length_append .. ▸ Nat.lt_add_right _ h) = l₁[n]
-| a :: l, _, 0, h => rfl
-| a :: l, _, n+1, h => by simp only [get, cons_append]; apply getElem_append
-
-@[deprecated getElem_append (since := "2024-06-12")]
-theorem get_append {l₁ l₂ : List α} (n : Nat) (h : n < l₁.length) :
-    (l₁ ++ l₂).get ⟨n, length_append .. ▸ Nat.lt_add_right _ h⟩ = l₁.get ⟨n, h⟩ := by
-  simp [getElem_append, h]
-
-@[deprecated getElem_append_left (since := "2024-06-12")]
-theorem get_append_left (as bs : List α) (h : i < as.length) {h'} : (as ++ bs).get ⟨i, h'⟩ = as.get ⟨i, h⟩ := by
-  simp [getElem_append_left, h, h']
-
-@[deprecated getElem_append_right (since := "2024-06-12")]
-theorem get_append_right (as bs : List α) (h : ¬ i < as.length) {h' h''} : (as ++ bs).get ⟨i, h'⟩ = bs.get ⟨i - as.length, h''⟩ := by
-  simp [getElem_append_right, h, h', h'']
-
-/-! ### map -/
-
-@[simp] theorem map_nil {f : α → β} : map f [] = [] := rfl
-
-@[simp] theorem map_cons (f : α → β) a l : map f (a :: l) = f a :: map f l := rfl
-
-@[simp] theorem map_append (f : α → β) : ∀ l₁ l₂, map f (l₁ ++ l₂) = map f l₁ ++ map f l₂ := by
-  intro l₁; induction l₁ <;> intros <;> simp_all
-
-@[simp] theorem map_id (l : List α) : map id l = l := by induction l <;> simp_all
-
-@[simp] theorem map_id' (l : List α) : map (fun a => a) l = l := by induction l <;> simp_all
-
-@[simp] theorem mem_map {f : α → β} : ∀ {l : List α}, b ∈ l.map f ↔ ∃ a, a ∈ l ∧ f a = b
-  | [] => by simp
-  | _ :: l => by simp [mem_map (l := l), eq_comm (a := b)]
-
-theorem mem_map_of_mem (f : α → β) (h : a ∈ l) : f a ∈ map f l := mem_map.2 ⟨_, h, rfl⟩
-
-@[simp] theorem map_map (g : β → γ) (f : α → β) (l : List α) :
-  map g (map f l) = map (g ∘ f) l := by induction l <;> simp_all
-
-/-! ### bind -/
-
-@[simp] theorem nil_bind (f : α → List β) : List.bind [] f = [] := by simp [join, List.bind]
-
-@[simp] theorem cons_bind x xs (f : α → List β) :
-  List.bind (x :: xs) f = f x ++ List.bind xs f := by simp [join, List.bind]
-
-@[simp] theorem append_bind xs ys (f : α → List β) :
-  List.bind (xs ++ ys) f = List.bind xs f ++ List.bind ys f := by
-  induction xs; {rfl}; simp_all [cons_bind, append_assoc]
-
-@[simp] theorem bind_id (l : List (List α)) : List.bind l id = l.join := by simp [List.bind]
-
-/-! ### join -/
-
-@[simp] theorem join_nil : List.join ([] : List (List α)) = [] := rfl
-
-@[simp] theorem join_cons : (l :: ls).join = l ++ ls.join := rfl
-
-/-! ### bounded quantifiers over Lists -/
+@[simp 1100] theorem mem_singleton {a b : α} : a ∈ [b] ↔ a = b :=
+  ⟨eq_of_mem_singleton, (by simp [·])⟩
 
 theorem forall_mem_cons {p : α → Prop} {a : α} {l : List α} :
     (∀ x, x ∈ a :: l → p x) ↔ p a ∧ ∀ x, x ∈ l → p x :=
   ⟨fun H => ⟨H _ (.head ..), fun _ h => H _ (.tail _ h)⟩,
    fun ⟨H₁, H₂⟩ _ => fun | .head .. => H₁ | .tail _ h => H₂ _ h⟩
 
-/-! ### reverse -/
+theorem exists_mem_nil (p : α → Prop) : ¬ (∃ x, ∃ _ : x ∈ @nil α, p x) := nofun
 
-@[simp] theorem reverseAux_nil : reverseAux [] r = r := rfl
-@[simp] theorem reverseAux_cons : reverseAux (a::l) r = reverseAux l (a::r) := rfl
+theorem forall_mem_nil (p : α → Prop) : ∀ (x) (_ : x ∈ @nil α), p x := nofun
 
-theorem reverseAux_eq (as bs : List α) : reverseAux as bs = reverse as ++ bs :=
-  reverseAux_eq_append ..
+theorem exists_mem_cons {p : α → Prop} {a : α} {l : List α} :
+    (∃ x, ∃ _ : x ∈ a :: l, p x) ↔ p a ∨ ∃ x, ∃ _ : x ∈ l, p x := by simp
 
-theorem reverse_map (f : α → β) (l : List α) : (l.map f).reverse = l.reverse.map f := by
-  induction l <;> simp [*]
+theorem forall_mem_singleton {p : α → Prop} {a : α} : (∀ (x) (_ : x ∈ [a]), p x) ↔ p a := by
+  simp only [mem_singleton, forall_eq]
 
-@[simp] theorem reverse_eq_nil_iff {xs : List α} : xs.reverse = [] ↔ xs = [] := by
-  match xs with
-  | [] => simp
-  | x :: xs => simp
+theorem mem_nil_iff (a : α) : a ∈ ([] : List α) ↔ False := by simp
 
-/-! ### nth element -/
+theorem mem_singleton_self (a : α) : a ∈ [a] := mem_cons_self _ _
+
+theorem mem_of_mem_cons_of_mem : ∀ {a b : α} {l : List α}, a ∈ b :: l → b ∈ l → a ∈ l
+  | _, _, _, .head .., h | _, _, _, .tail _ h, _ => h
+
+theorem eq_or_ne_mem_of_mem {a b : α} {l : List α} (h' : a ∈ b :: l) : a = b ∨ (a ≠ b ∧ a ∈ l) :=
+  (Classical.em _).imp_right fun h => ⟨h, (mem_cons.1 h').resolve_left h⟩
+
+theorem ne_nil_of_mem {a : α} {l : List α} (h : a ∈ l) : l ≠ [] := by cases h <;> nofun
+
+theorem elem_iff [BEq α] [LawfulBEq α] {a : α} {as : List α} :
+    elem a as = true ↔ a ∈ as := ⟨mem_of_elem_eq_true, elem_eq_true_of_mem⟩
+
+@[simp] theorem elem_eq_mem [BEq α] [LawfulBEq α] (a : α) (as : List α) :
+    elem a as = decide (a ∈ as) := by rw [Bool.eq_iff_iff, elem_iff, decide_eq_true_iff]
+
+theorem mem_of_ne_of_mem {a y : α} {l : List α} (h₁ : a ≠ y) (h₂ : a ∈ y :: l) : a ∈ l :=
+  Or.elim (mem_cons.mp h₂) (absurd · h₁) (·)
+
+theorem ne_of_not_mem_cons {a b : α} {l : List α} : a ∉ b::l → a ≠ b := mt (· ▸ .head _)
+
+theorem not_mem_of_not_mem_cons {a b : α} {l : List α} : a ∉ b::l → a ∉ l := mt (.tail _)
+
+theorem not_mem_cons_of_ne_of_not_mem {a y : α} {l : List α} : a ≠ y → a ∉ l → a ∉ y::l :=
+  mt ∘ mem_of_ne_of_mem
+
+theorem ne_and_not_mem_of_not_mem_cons {a y : α} {l : List α} : a ∉ y::l → a ≠ y ∧ a ∉ l :=
+  fun p => ⟨ne_of_not_mem_cons p, not_mem_of_not_mem_cons p⟩
 
 theorem getElem_of_mem : ∀ {a} {l : List α}, a ∈ l → ∃ (n : Nat) (h : n < l.length), l[n]'h = a
   | _, _ :: _, .head .. => ⟨0, Nat.succ_pos _, rfl⟩
@@ -264,567 +367,25 @@ theorem mem_iff_getElem {a} {l : List α} : a ∈ l ↔ ∃ (n : Nat) (h : n < l
 theorem mem_iff_get {a} {l : List α} : a ∈ l ↔ ∃ n, get l n = a :=
   ⟨get_of_mem, fun ⟨_, e⟩ => e ▸ get_mem ..⟩
 
-@[simp] theorem getElem?_map (f : α → β) : ∀ (l : List α) (n : Nat), (map f l)[n]? = Option.map f l[n]?
-  | [], _ => rfl
-  | _ :: _, 0 => by simp
-  | _ :: l, n+1 => by simp [getElem?_map f l n]
+theorem getElem?_of_mem {a} {l : List α} (h : a ∈ l) : ∃ n : Nat, l[n]? = some a :=
+  let ⟨n, _, e⟩ := getElem_of_mem h; ⟨n, e ▸ getElem?_eq_getElem _⟩
 
-@[deprecated getElem?_map (since := "2024-06-12")]
-theorem get?_map (f : α → β) : ∀ l n, (map f l).get? n = (l.get? n).map f
-  | [], _ => rfl
-  | _ :: _, 0 => rfl
-  | _ :: l, n+1 => get?_map f l n
+theorem get?_of_mem {a} {l : List α} (h : a ∈ l) : ∃ n, l.get? n = some a :=
+  let ⟨⟨n, _⟩, e⟩ := get_of_mem h; ⟨n, e ▸ get?_eq_get _⟩
 
-theorem getElem?_append {l₁ l₂ : List α} {n : Nat} (hn : n < l₁.length) :
-    (l₁ ++ l₂)[n]? = l₁[n]? := by
-  have hn' : n < (l₁ ++ l₂).length := Nat.lt_of_lt_of_le hn <|
-    length_append .. ▸ Nat.le_add_right ..
-  simp_all [getElem?_eq_getElem, getElem_append]
+theorem getElem?_mem {l : List α} {n : Nat} {a : α} (e : l[n]? = some a) : a ∈ l :=
+  let ⟨_, e⟩ := getElem?_eq_some.1 e; e ▸ getElem_mem ..
 
-@[deprecated (since := "2024-06-12")]
-theorem get?_append {l₁ l₂ : List α} {n : Nat} (hn : n < l₁.length) :
-    (l₁ ++ l₂).get? n = l₁.get? n := by
-  simp [getElem?_append hn]
+theorem get?_mem {l : List α} {n a} (e : l.get? n = some a) : a ∈ l :=
+  let ⟨_, e⟩ := get?_eq_some.1 e; e ▸ get_mem ..
 
-@[simp] theorem getElem?_concat_length : ∀ (l : List α) (a : α), (l ++ [a])[l.length]? = some a
-  | [], a => rfl
-  | b :: l, a => by rw [cons_append, length_cons]; simp [getElem?_concat_length]
+theorem mem_iff_getElem? {a} {l : List α} : a ∈ l ↔ ∃ n : Nat, l[n]? = some a := by
+  simp [getElem?_eq_some, mem_iff_getElem]
 
-@[deprecated getElem?_concat_length (since := "2024-06-12")]
-theorem get?_concat_length (l : List α) (a : α) : (l ++ [a]).get? l.length = some a := by simp
+theorem mem_iff_get? {a} {l : List α} : a ∈ l ↔ ∃ n, l.get? n = some a := by
+  simp [getElem?_eq_some, Fin.exists_iff, mem_iff_get]
 
-theorem getLast_eq_get : ∀ (l : List α) (h : l ≠ []),
-    getLast l h = l.get ⟨l.length - 1, by
-      match l with
-      | [] => contradiction
-      | a :: l => exact Nat.le_refl _⟩
-  | [a], h => rfl
-  | a :: b :: l, h => by
-    simp [getLast, get, Nat.succ_sub_succ, getLast_eq_get]
-
-@[simp] theorem getLast?_nil : @getLast? α [] = none := rfl
-
-theorem getLast?_eq_getLast : ∀ l h, @getLast? α l = some (getLast l h)
-  | [], h => nomatch h rfl
-  | _::_, _ => rfl
-
-theorem getLast?_eq_get? : ∀ (l : List α), getLast? l = l.get? (l.length - 1)
-  | [] => rfl
-  | a::l => by rw [getLast?_eq_getLast (a::l) nofun, getLast_eq_get, get?_eq_get]
-
-@[simp] theorem getLast?_concat (l : List α) : getLast? (l ++ [a]) = some a := by
-  simp [getLast?_eq_get?, Nat.succ_sub_succ]
-
-@[simp] theorem getD_eq_getElem? (l) (n) (a : α) : getD l n a = (l[n]?).getD a := by
-  simp [getD]
-
-@[deprecated getD_eq_getElem? (since := "2024-06-12")]
-theorem getD_eq_get? : ∀ l n (a : α), getD l n a = (get? l n).getD a := by simp
-
-theorem getElem?_append_right : ∀ {l₁ l₂ : List α} {n : Nat}, l₁.length ≤ n →
-  (l₁ ++ l₂)[n]? = l₂[n - l₁.length]?
-| [], _, n, _ => rfl
-| a :: l, _, n+1, h₁ => by
-  rw [cons_append]
-  simp [Nat.succ_sub_succ_eq_sub, getElem?_append_right (Nat.lt_succ.1 h₁)]
-
-@[deprecated getElem?_append_right (since := "2024-06-12")]
-theorem get?_append_right {l₁ l₂ : List α} {n : Nat} (h : l₁.length ≤ n) :
-    (l₁ ++ l₂).get? n = l₂.get? (n - l₁.length) := by
-  simp [getElem?_append_right, h]
-
-theorem getElem?_reverse' : ∀ {l : List α} (i j), i + j + 1 = length l →
-    l.reverse[i]? = l[j]?
-  | [], _, _, _ => rfl
-  | a::l, i, 0, h => by simp [Nat.succ.injEq] at h; simp [h, getElem?_append_right, Nat.succ.injEq]
-  | a::l, i, j+1, h => by
-    have := Nat.succ.inj h; simp at this ⊢
-    rw [getElem?_append, getElem?_reverse' _ _ this]
-    rw [length_reverse, ← this]; apply Nat.lt_add_of_pos_right (Nat.succ_pos _)
-
-@[deprecated getElem?_reverse' (since := "2024-06-12")]
-theorem get?_reverse' {l : List α} (i j) (h : i + j + 1 = length l) : get? l.reverse i = get? l j := by
-  simp [getElem?_reverse' _ _ h]
-
-theorem getElem?_reverse {l : List α} {i} (h : i < length l) :
-    l.reverse[i]? = l[l.length - 1 - i]? :=
-  getElem?_reverse' _ _ <| by
-    rw [Nat.add_sub_of_le (Nat.le_sub_one_of_lt h),
-      Nat.sub_add_cancel (Nat.lt_of_le_of_lt (Nat.zero_le _) h)]
-
-@[deprecated getElem?_reverse (since := "2024-06-12")]
-theorem get?_reverse {l : List α} {i} (h : i < length l) :
-    get? l.reverse i = get? l (l.length - 1 - i) := by
-  simp [getElem?_reverse h]
-
-@[simp] theorem getD_nil : getD [] n d = d := rfl
-
-@[simp] theorem getD_cons_zero : getD (x :: xs) 0 d = x := rfl
-
-@[simp] theorem getD_cons_succ : getD (x :: xs) (n + 1) d = getD xs n d := rfl
-
-@[ext] theorem ext_getElem? {l₁ l₂ : List α} (h : ∀ n : Nat, l₁[n]? = l₂[n]?) : l₁ = l₂ :=
-  ext_get? fun n => by simp_all
-
-theorem ext_getElem {l₁ l₂ : List α} (hl : length l₁ = length l₂)
-    (h : ∀ (n : Nat) (h₁ : n < l₁.length) (h₂ : n < l₂.length), l₁[n]'h₁ = l₂[n]'h₂) : l₁ = l₂ :=
-  ext_getElem? fun n =>
-    if h₁ : n < length l₁ then by
-      simp_all [getElem?_eq_getElem]
-    else by
-      have h₁ := Nat.le_of_not_lt h₁
-      rw [getElem?_len_le h₁, getElem?_len_le]; rwa [← hl]
-
-theorem ext_get {l₁ l₂ : List α} (hl : length l₁ = length l₂)
-    (h : ∀ n h₁ h₂, get l₁ ⟨n, h₁⟩ = get l₂ ⟨n, h₂⟩) : l₁ = l₂ :=
-  ext_getElem hl (by simp_all)
-
-@[simp] theorem getElem_map (f : α → β) {l} {n : Nat} {h : n < (map f l).length} :
-    (map f l)[n] = f (l[n]'(length_map l f ▸ h)) :=
-  Option.some.inj <| by rw [← getElem?_eq_getElem, getElem?_map, getElem?_eq_getElem]; rfl
-
-@[deprecated getElem_map (since := "2024-06-12")]
-theorem get_map (f : α → β) {l n} :
-    get (map f l) n = f (get l ⟨n, length_map l f ▸ n.2⟩) := by
-  simp
-
-/-! ### take and drop -/
-
-@[simp] theorem take_append_drop : ∀ (n : Nat) (l : List α), take n l ++ drop n l = l
-  | 0, _ => rfl
-  | _+1, [] => rfl
-  | n+1, x :: xs => congrArg (cons x) <| take_append_drop n xs
-
-@[simp] theorem length_drop : ∀ (i : Nat) (l : List α), length (drop i l) = length l - i
-  | 0, _ => rfl
-  | succ i, [] => Eq.symm (Nat.zero_sub (succ i))
-  | succ i, x :: l => calc
-    length (drop (succ i) (x :: l)) = length l - i := length_drop i l
-    _ = succ (length l) - succ i := (Nat.succ_sub_succ_eq_sub (length l) i).symm
-
-theorem drop_length_le {l : List α} (h : l.length ≤ i) : drop i l = [] :=
-  length_eq_zero.1 (length_drop .. ▸ Nat.sub_eq_zero_of_le h)
-
-theorem take_length_le {l : List α} (h : l.length ≤ i) : take i l = l := by
-  have := take_append_drop i l
-  rw [drop_length_le h, append_nil] at this; exact this
-
-@[simp] theorem take_zero (l : List α) : l.take 0 = [] := rfl
-
-@[simp] theorem take_nil : ([] : List α).take i = [] := by cases i <;> rfl
-
-@[simp] theorem take_cons_succ : (a::as).take (i+1) = a :: as.take i := rfl
-
-@[simp] theorem drop_zero (l : List α) : l.drop 0 = l := rfl
-
-@[simp] theorem drop_succ_cons : (a :: l).drop (n + 1) = l.drop n := rfl
-
-@[simp] theorem drop_length (l : List α) : drop l.length l = [] := drop_length_le (Nat.le_refl _)
-
-@[simp] theorem take_length (l : List α) : take l.length l = l := take_length_le (Nat.le_refl _)
-
-theorem take_concat_get (l : List α) (i : Nat) (h : i < l.length) :
-    (l.take i).concat l[i] = l.take (i+1) :=
-  Eq.symm <| (append_left_inj _).1 <| (take_append_drop (i+1) l).trans <| by
-    rw [concat_eq_append, append_assoc, singleton_append, get_drop_eq_drop, take_append_drop]
-
-theorem reverse_concat (l : List α) (a : α) : (l.concat a).reverse = a :: l.reverse := by
-  rw [concat_eq_append, reverse_append]; rfl
-
-/-! ### takeWhile and dropWhile -/
-
-@[simp] theorem dropWhile_nil : ([] : List α).dropWhile p = [] := rfl
-
-theorem dropWhile_cons :
-    (x :: xs : List α).dropWhile p = if p x then xs.dropWhile p else x :: xs := by
-  split <;> simp_all [dropWhile]
-
-/-! ### foldlM and foldrM -/
-
-@[simp] theorem foldlM_reverse [Monad m] (l : List α) (f : β → α → m β) (b) :
-    l.reverse.foldlM f b = l.foldrM (fun x y => f y x) b := rfl
-
-@[simp] theorem foldlM_nil [Monad m] (f : β → α → m β) (b) : [].foldlM f b = pure b := rfl
-
-@[simp] theorem foldlM_cons [Monad m] (f : β → α → m β) (b) (a) (l : List α) :
-    (a :: l).foldlM f b = f b a >>= l.foldlM f := by
-  simp [List.foldlM]
-
-@[simp] theorem foldlM_append [Monad m] [LawfulMonad m] (f : β → α → m β) (b) (l l' : List α) :
-    (l ++ l').foldlM f b = l.foldlM f b >>= l'.foldlM f := by
-  induction l generalizing b <;> simp [*]
-
-@[simp] theorem foldrM_nil [Monad m] (f : α → β → m β) (b) : [].foldrM f b = pure b := rfl
-
-@[simp] theorem foldrM_cons [Monad m] [LawfulMonad m] (a : α) (l) (f : α → β → m β) (b) :
-    (a :: l).foldrM f b = l.foldrM f b >>= f a := by
-  simp only [foldrM]
-  induction l <;> simp_all
-
-@[simp] theorem foldrM_reverse [Monad m] (l : List α) (f : α → β → m β) (b) :
-    l.reverse.foldrM f b = l.foldlM (fun x y => f y x) b :=
-  (foldlM_reverse ..).symm.trans <| by simp
-
-theorem foldl_eq_foldlM (f : β → α → β) (b) (l : List α) :
-    l.foldl f b = l.foldlM (m := Id) f b := by
-  induction l generalizing b <;> simp [*, foldl]
-
-theorem foldr_eq_foldrM (f : α → β → β) (b) (l : List α) :
-    l.foldr f b = l.foldrM (m := Id) f b := by
-  induction l <;> simp [*, foldr]
-
-/-! ### foldl and foldr -/
-
-@[simp] theorem foldl_reverse (l : List α) (f : β → α → β) (b) :
-    l.reverse.foldl f b = l.foldr (fun x y => f y x) b := by simp [foldl_eq_foldlM, foldr_eq_foldrM]
-
-@[simp] theorem foldr_reverse (l : List α) (f : α → β → β) (b) :
-    l.reverse.foldr f b = l.foldl (fun x y => f y x) b :=
-  (foldl_reverse ..).symm.trans <| by simp
-
-@[simp] theorem foldrM_append [Monad m] [LawfulMonad m] (f : α → β → m β) (b) (l l' : List α) :
-    (l ++ l').foldrM f b = l'.foldrM f b >>= l.foldrM f := by
-  induction l <;> simp [*]
-
-@[simp] theorem foldl_append {β : Type _} (f : β → α → β) (b) (l l' : List α) :
-    (l ++ l').foldl f b = l'.foldl f (l.foldl f b) := by simp [foldl_eq_foldlM]
-
-@[simp] theorem foldr_append (f : α → β → β) (b) (l l' : List α) :
-    (l ++ l').foldr f b = l.foldr f (l'.foldr f b) := by simp [foldr_eq_foldrM]
-
-@[simp] theorem foldl_nil : [].foldl f b = b := rfl
-
-@[simp] theorem foldl_cons (l : List α) (b : β) : (a :: l).foldl f b = l.foldl f (f b a) := rfl
-
-@[simp] theorem foldr_nil : [].foldr f b = b := rfl
-
-@[simp] theorem foldr_cons (l : List α) : (a :: l).foldr f b = f a (l.foldr f b) := rfl
-
-@[simp] theorem foldr_self_append (l : List α) : l.foldr cons l' = l ++ l' := by
-  induction l <;> simp [*]
-
-theorem foldr_self (l : List α) : l.foldr cons [] = l := by simp
-
-theorem foldl_map (f : β₁ → β₂) (g : α → β₂ → α) (l : List β₁) (init : α) :
-    (l.map f).foldl g init = l.foldl (fun x y => g x (f y)) init := by
-  induction l generalizing init <;> simp [*]
-
-theorem foldr_map (f : α₁ → α₂) (g : α₂ → β → β) (l : List α₁) (init : β) :
-    (l.map f).foldr g init = l.foldr (fun x y => g (f x) y) init := by
-  induction l generalizing init <;> simp [*]
-
-/-! ### mapM -/
-
-/-- Alternate (non-tail-recursive) form of mapM for proofs. -/
-def mapM' [Monad m] (f : α → m β) : List α → m (List β)
-  | [] => pure []
-  | a :: l => return (← f a) :: (← l.mapM' f)
-
-@[simp] theorem mapM'_nil [Monad m] {f : α → m β} : mapM' f [] = pure [] := rfl
-@[simp] theorem mapM'_cons [Monad m] {f : α → m β} :
-    mapM' f (a :: l) = return ((← f a) :: (← l.mapM' f)) :=
-  rfl
-
-theorem mapM'_eq_mapM [Monad m] [LawfulMonad m] (f : α → m β) (l : List α) :
-    mapM' f l = mapM f l := by simp [go, mapM] where
-  go : ∀ l acc, mapM.loop f l acc = return acc.reverse ++ (← mapM' f l)
-    | [], acc => by simp [mapM.loop, mapM']
-    | a::l, acc => by simp [go l, mapM.loop, mapM']
-
-@[simp] theorem mapM_nil [Monad m] (f : α → m β) : [].mapM f = pure [] := rfl
-
-@[simp] theorem mapM_cons [Monad m] [LawfulMonad m] (f : α → m β) :
-    (a :: l).mapM f = (return (← f a) :: (← l.mapM f)) := by simp [← mapM'_eq_mapM, mapM']
-
-@[simp] theorem mapM_append [Monad m] [LawfulMonad m] (f : α → m β) {l₁ l₂ : List α} :
-    (l₁ ++ l₂).mapM f = (return (← l₁.mapM f) ++ (← l₂.mapM f)) := by induction l₁ <;> simp [*]
-
-/-! ### forM -/
-
--- We use `List.forM` as the simp normal form, rather that `ForM.forM`.
--- As such we need to replace `List.forM_nil` and `List.forM_cons`:
-
-@[simp] theorem forM_nil' [Monad m] : ([] : List α).forM f = (pure .unit : m PUnit) := rfl
-
-@[simp] theorem forM_cons' [Monad m] :
-    (a::as).forM f = (f a >>= fun _ => as.forM f : m PUnit) :=
-  List.forM_cons _ _ _
-
-/-! ### eraseIdx -/
-
-@[simp] theorem eraseIdx_nil : ([] : List α).eraseIdx i = [] := rfl
-@[simp] theorem eraseIdx_cons_zero : (a::as).eraseIdx 0 = as := rfl
-@[simp] theorem eraseIdx_cons_succ : (a::as).eraseIdx (i+1) = a :: as.eraseIdx i := rfl
-
-/-! ### find? -/
-
-@[simp] theorem find?_nil : ([] : List α).find? p = none := rfl
-theorem find?_cons : (a::as).find? p = match p a with | true => some a | false => as.find? p :=
-  rfl
-
-/-! ### filter -/
-
-@[simp] theorem filter_nil (p : α → Bool) : filter p [] = [] := rfl
-
-@[simp] theorem filter_cons_of_pos {p : α → Bool} {a : α} (l) (pa : p a) :
-    filter p (a :: l) = a :: filter p l := by rw [filter, pa]
-
-@[simp] theorem filter_cons_of_neg {p : α → Bool} {a : α} (l) (pa : ¬ p a) :
-    filter p (a :: l) = filter p l := by rw [filter, eq_false_of_ne_true pa]
-
-theorem filter_cons :
-    (x :: xs : List α).filter p = if p x then x :: (xs.filter p) else xs.filter p := by
-  split <;> simp [*]
-
-theorem mem_filter : x ∈ filter p as ↔ x ∈ as ∧ p x := by
-  induction as with
-  | nil => simp [filter]
-  | cons a as ih =>
-    by_cases h : p a
-    · simp_all [or_and_left]
-    · simp_all [or_and_right]
-
-theorem filter_eq_nil {l} : filter p l = [] ↔ ∀ a, a ∈ l → ¬p a := by
-  simp only [eq_nil_iff_forall_not_mem, mem_filter, not_and]
-
-/-! ### findSome? -/
-
-@[simp] theorem findSome?_nil : ([] : List α).findSome? f = none := rfl
-
-theorem findSome?_cons {f : α → Option β} :
-    (a::as).findSome? f = match f a with | some b => some b | none => as.findSome? f :=
-  rfl
-
-/-! ### replace -/
-
-@[simp] theorem replace_nil [BEq α] : ([] : List α).replace a b = [] := rfl
-
-theorem replace_cons [BEq α] {a : α} :
-    (a::as).replace b c = match a == b with | true => c::as | false => a :: replace as b c :=
-  rfl
-
-@[simp] theorem replace_cons_self [BEq α] [LawfulBEq α] {a : α} : (a::as).replace a b = b::as := by
-  simp [replace_cons]
-
-/-! ### elem -/
-
-@[simp] theorem elem_nil [BEq α] : ([] : List α).elem a = false := rfl
-
-theorem elem_cons [BEq α] {a : α} :
-    (a::as).elem b = match a == b with | true => true | false => as.elem b := rfl
-
-@[simp] theorem elem_cons_self [BEq α] [LawfulBEq α] {a : α} : (a::as).elem a = true := by
-  simp [elem_cons]
-
-/-! ### lookup -/
-
-@[simp] theorem lookup_nil [BEq α] : ([] : List (α × β)).lookup a = none := rfl
-
-theorem lookup_cons [BEq α] {k : α} :
-    ((k,b)::es).lookup a = match a == k with | true => some b | false => es.lookup a :=
-  rfl
-
-@[simp] theorem lookup_cons_self [BEq α] [LawfulBEq α] {k : α} : ((k,b)::es).lookup k = some b := by
-  simp [lookup_cons]
-
-/-! ### zipWith -/
-
-@[simp] theorem zipWith_nil_left {f : α → β → γ} : zipWith f [] l = [] := by
-  rfl
-
-@[simp] theorem zipWith_nil_right {f : α → β → γ} : zipWith f l [] = [] := by
-  simp [zipWith]
-
-@[simp] theorem zipWith_cons_cons {f : α → β → γ} :
-    zipWith f (a :: as) (b :: bs) = f a b :: zipWith f as bs := by
-  rfl
-
-theorem getElem?_zipWith {f : α → β → γ} {i : Nat} :
-    (List.zipWith f as bs)[i]? = match as[i]?, bs[i]? with
-      | some a, some b => some (f a b) | _, _ => none := by
-  induction as generalizing bs i with
-  | nil => cases bs with
-    | nil => simp
-    | cons b bs => simp
-  | cons a as aih => cases bs with
-    | nil => simp
-    | cons b bs => cases i <;> simp_all
-
-@[deprecated getElem?_zipWith (since := "2024-06-12")]
-theorem get?_zipWith {f : α → β → γ} :
-    (List.zipWith f as bs).get? i = match as.get? i, bs.get? i with
-      | some a, some b => some (f a b) | _, _ => none := by
-  simp [getElem?_zipWith]
-
-set_option linter.deprecated false in
-@[deprecated getElem?_zipWith (since := "2024-06-07")] abbrev zipWith_get? := @get?_zipWith
-
-/-! ### zipWithAll -/
-
-theorem getElem?_zipWithAll {f : Option α → Option β → γ} {i : Nat } :
-    (zipWithAll f as bs)[i]? = match as[i]?, bs[i]? with
-      | none, none => .none | a?, b? => some (f a? b?) := by
-  induction as generalizing bs i with
-  | nil => induction bs generalizing i with
-    | nil => simp
-    | cons b bs bih => cases i <;> simp_all
-  | cons a as aih => cases bs with
-    | nil =>
-      specialize @aih []
-      cases i <;> simp_all
-    | cons b bs => cases i <;> simp_all
-
-@[deprecated getElem?_zipWithAll (since := "2024-06-12")]
-theorem get?_zipWithAll {f : Option α → Option β → γ} :
-    (zipWithAll f as bs).get? i = match as.get? i, bs.get? i with
-      | none, none => .none | a?, b? => some (f a? b?) := by
-  simp [getElem?_zipWithAll]
-
-set_option linter.deprecated false in
-@[deprecated getElem?_zipWithAll (since := "2024-06-07")] abbrev zipWithAll_get? := @get?_zipWithAll
-
-/-! ### zip -/
-
-@[simp] theorem zip_nil_left : zip ([] : List α) (l : List β)  = [] := by
-  rfl
-
-@[simp] theorem zip_nil_right : zip (l : List α) ([] : List β)  = [] := by
-  simp [zip]
-
-@[simp] theorem zip_cons_cons : zip (a :: as) (b :: bs) = (a, b) :: zip as bs := by
-  rfl
-
-/-! ### unzip -/
-
-@[simp] theorem unzip_nil : ([] : List (α × β)).unzip = ([], []) := rfl
-
-@[simp] theorem unzip_cons {h : α × β} :
-    (h :: t).unzip = match unzip t with | (al, bl) => (h.1::al, h.2::bl) := rfl
-
-/-! ### all / any -/
-
-@[simp] theorem all_eq_true {l : List α} : l.all p ↔ ∀ x, x ∈ l →  p x := by induction l <;> simp [*]
-
-@[simp] theorem any_eq_true {l : List α} : l.any p ↔ ∃ x, x ∈ l ∧ p x := by induction l <;> simp [*]
-
-/-! ### enumFrom -/
-
-@[simp] theorem enumFrom_nil : ([] : List α).enumFrom i = [] := rfl
-@[simp] theorem enumFrom_cons : (a::as).enumFrom i = (i, a) :: as.enumFrom (i+1) := rfl
-
-/-! ### iota -/
-
-@[simp] theorem iota_zero : iota 0 = [] := rfl
-@[simp] theorem iota_succ : iota (i+1) = (i+1) :: iota i := rfl
-
-/-! ### intersperse -/
-
-@[simp] theorem intersperse_nil (sep : α) : ([] : List α).intersperse sep = [] := rfl
-@[simp] theorem intersperse_single (sep : α) : [x].intersperse sep = [x] := rfl
-@[simp] theorem intersperse_cons₂ (sep : α) :
-    (x::y::zs).intersperse sep = x::sep::((y::zs).intersperse sep) := rfl
-
-/-! ### isPrefixOf -/
-
-@[simp] theorem isPrefixOf_nil_left [BEq α] : isPrefixOf ([] : List α) l = true := by
-  simp [isPrefixOf]
-@[simp] theorem isPrefixOf_cons_nil [BEq α] : isPrefixOf (a::as) ([] : List α) = false := rfl
-theorem isPrefixOf_cons₂ [BEq α] {a : α} :
-    isPrefixOf (a::as) (b::bs) = (a == b && isPrefixOf as bs) := rfl
-@[simp] theorem isPrefixOf_cons₂_self [BEq α] [LawfulBEq α] {a : α} :
-    isPrefixOf (a::as) (a::bs) = isPrefixOf as bs := by simp [isPrefixOf_cons₂]
-
-/-! ### isEqv -/
-
-@[simp] theorem isEqv_nil_nil : isEqv ([] : List α) [] eqv = true := rfl
-@[simp] theorem isEqv_nil_cons : isEqv ([] : List α) (a::as) eqv = false := rfl
-@[simp] theorem isEqv_cons_nil : isEqv (a::as : List α) [] eqv = false := rfl
-theorem isEqv_cons₂ : isEqv (a::as) (b::bs) eqv = (eqv a b && isEqv as bs eqv) := rfl
-
-/-! ### dropLast -/
-
-@[simp] theorem dropLast_nil : ([] : List α).dropLast = [] := rfl
-@[simp] theorem dropLast_single : [x].dropLast = [] := rfl
-@[simp] theorem dropLast_cons₂ :
-    (x::y::zs).dropLast = x :: (y::zs).dropLast := rfl
-
--- We may want to replace these `simp` attributes with explicit equational lemmas,
--- as we already have for all the non-monadic functions.
-attribute [simp] mapA forA filterAuxM firstM anyM allM findM? findSomeM?
-
--- Previously `range.loop`, `mapM.loop`, `filterMapM.loop`, `forIn.loop`, `forIn'.loop`
--- had attribute `@[simp]`.
--- We don't currently provide simp lemmas,
--- as this is an internal implementation and they don't seem to be needed.
-
-/-! ### minimum? -/
-
-@[simp] theorem minimum?_nil [Min α] : ([] : List α).minimum? = none := rfl
-
--- We don't put `@[simp]` on `minimum?_cons`,
--- because the definition in terms of `foldl` is not useful for proofs.
-theorem minimum?_cons [Min α] {xs : List α} : (x :: xs).minimum? = foldl min x xs := rfl
-
-@[simp] theorem minimum?_eq_none_iff {xs : List α} [Min α] : xs.minimum? = none ↔ xs = [] := by
-  cases xs <;> simp [minimum?]
-
-theorem minimum?_mem [Min α] (min_eq_or : ∀ a b : α, min a b = a ∨ min a b = b) :
-    {xs : List α} → xs.minimum? = some a → a ∈ xs := by
-  intro xs
-  match xs with
-  | nil => simp
-  | x :: xs =>
-    simp only [minimum?_cons, Option.some.injEq, List.mem_cons]
-    intro eq
-    induction xs generalizing x with
-    | nil =>
-      simp at eq
-      simp [eq]
-    | cons y xs ind =>
-      simp at eq
-      have p := ind _ eq
-      cases p with
-      | inl p =>
-        cases min_eq_or x y with | _ q => simp [p, q]
-      | inr p => simp [p, mem_cons]
-
-theorem le_minimum?_iff [Min α] [LE α]
-    (le_min_iff : ∀ a b c : α, a ≤ min b c ↔ a ≤ b ∧ a ≤ c) :
-    {xs : List α} → xs.minimum? = some a → ∀ x, x ≤ a ↔ ∀ b, b ∈ xs → x ≤ b
-  | nil => by simp
-  | cons x xs => by
-    rw [minimum?]
-    intro eq y
-    simp only [Option.some.injEq] at eq
-    induction xs generalizing x with
-    | nil =>
-      simp at eq
-      simp [eq]
-    | cons z xs ih =>
-      simp at eq
-      simp [ih _ eq, le_min_iff, and_assoc]
-
--- This could be refactored by designing appropriate typeclasses to replace `le_refl`, `min_eq_or`,
--- and `le_min_iff`.
-theorem minimum?_eq_some_iff [Min α] [LE α] [anti : Antisymm ((· : α) ≤ ·)]
-    (le_refl : ∀ a : α, a ≤ a)
-    (min_eq_or : ∀ a b : α, min a b = a ∨ min a b = b)
-    (le_min_iff : ∀ a b c : α, a ≤ min b c ↔ a ≤ b ∧ a ≤ c) {xs : List α} :
-    xs.minimum? = some a ↔ a ∈ xs ∧ ∀ b, b ∈ xs → a ≤ b := by
-  refine ⟨fun h => ⟨minimum?_mem min_eq_or h, (le_minimum?_iff le_min_iff h _).1 (le_refl _)⟩, ?_⟩
-  intro ⟨h₁, h₂⟩
-  cases xs with
-  | nil => simp at h₁
-  | cons x xs =>
-    exact congrArg some <| anti.1
-      ((le_minimum?_iff le_min_iff (xs := x::xs) rfl _).1 (le_refl _) _ h₁)
-      (h₂ _ (minimum?_mem min_eq_or (xs := x::xs) rfl))
-
-@[simp] theorem get_cons_succ {as : List α} {h : i + 1 < (a :: as).length} :
-  (a :: as).get ⟨i+1, h⟩ = as.get ⟨i, Nat.lt_of_succ_lt_succ h⟩ := rfl
-
-@[simp] theorem get_cons_succ' {as : List α} {i : Fin as.length} :
-  (a :: as).get i.succ = as.get i := rfl
+/-! ### set -/
 
 @[simp] theorem set_nil (n : Nat) (a : α) : [].set n a = [] := rfl
 
@@ -832,7 +393,7 @@ theorem minimum?_eq_some_iff [Min α] [LE α] [anti : Antisymm ((· : α) ≤ ·
   (x :: xs).set 0 a = a :: xs := rfl
 
 @[simp] theorem set_succ (x : α) (xs : List α) (n : Nat) (a : α) :
-  (x :: xs).set n.succ a = x :: xs.set n a := rfl
+  (x :: xs).set (n + 1) a = x :: xs.set n a := rfl
 
 @[simp] theorem getElem_set_eq (l : List α) (i : Nat) (a : α) (h : i < (l.set i a).length) :
     (l.set i a)[i] = a :=
@@ -872,123 +433,504 @@ theorem get_set_ne (l : List α) {i j : Nat} (h : i ≠ j) (a : α)
     (l.set i a).get ⟨j, hj⟩ = l.get ⟨j, by simp at hj; exact hj⟩ := by
   simp [h]
 
-open Nat
+@[simp] theorem set_eq_nil (l : List α) (n : Nat) (a : α) : l.set n a = [] ↔ l = [] := by
+  cases l <;> cases n <;> simp only [set]
 
-/-! # Basic properties of Lists -/
-
-theorem cons_ne_nil (a : α) (l : List α) : a :: l ≠ [] := nofun
+theorem set_comm (a b : α) : ∀ {n m : Nat} (l : List α), n ≠ m →
+    (l.set n a).set m b = (l.set m b).set n a
+  | _, _, [], _ => by simp
+  | n+1, 0, _ :: _, _ => by simp [set]
+  | 0, m+1, _ :: _, _ => by simp [set]
+  | n+1, m+1, x :: t, h =>
+    congrArg _ <| set_comm a b t fun h' => h <| Nat.succ_inj'.mpr h'
 
 @[simp]
-theorem cons_ne_self (a : α) (l : List α) : a :: l ≠ l := mt (congrArg length) (Nat.succ_ne_self _)
+theorem set_set (a b : α) : ∀ (l : List α) (n : Nat), (l.set n a).set n b = l.set n b
+  | [], _ => by simp
+  | _ :: _, 0 => by simp [set]
+  | _ :: _, _+1 => by simp [set, set_set]
 
-theorem head_eq_of_cons_eq (H : h₁ :: t₁ = h₂ :: t₂) : h₁ = h₂ := (cons.inj H).1
+theorem getElem_set (a : α) {m n} (l : List α) (h) :
+    (set l m a)[n]'h = if m = n then a else l[n]'(length_set .. ▸ h) := by
+  if h : m = n then
+    subst m; simp only [getElem_set_eq, ↓reduceIte]
+  else
+    simp [h]
 
-theorem tail_eq_of_cons_eq (H : h₁ :: t₁ = h₂ :: t₂) : t₁ = t₂ := (cons.inj H).2
+@[deprecated getElem_set (since := "2024-06-12")]
+theorem get_set (a : α) {m n} (l : List α) (h) :
+    (set l m a).get ⟨n, h⟩ = if m = n then a else l.get ⟨n, length_set .. ▸ h⟩ := by
+  simp [getElem_set]
 
-theorem cons_inj (a : α) {l l' : List α} : a :: l = a :: l' ↔ l = l' :=
-  ⟨tail_eq_of_cons_eq, congrArg _⟩
+theorem mem_or_eq_of_mem_set : ∀ {l : List α} {n : Nat} {a b : α}, a ∈ l.set n b → a ∈ l ∨ a = b
+  | _ :: _, 0, _, _, h => ((mem_cons ..).1 h).symm.imp_left (.tail _)
+  | _ :: _, _+1, _, _, .head .. => .inl (.head ..)
+  | _ :: _, _+1, _, _, .tail _ h => (mem_or_eq_of_mem_set h).imp_left (.tail _)
 
-theorem cons_eq_cons {a b : α} {l l' : List α} : a :: l = b :: l' ↔ a = b ∧ l = l' :=
-  List.cons.injEq .. ▸ .rfl
+/-! ### foldlM and foldrM -/
 
-theorem exists_cons_of_ne_nil : ∀ {l : List α}, l ≠ [] → ∃ b L, l = b :: L
-  | c :: l', _ => ⟨c, l', rfl⟩
+@[simp] theorem foldlM_reverse [Monad m] (l : List α) (f : β → α → m β) (b) :
+    l.reverse.foldlM f b = l.foldrM (fun x y => f y x) b := rfl
 
-/-! ### length -/
+@[simp] theorem foldlM_append [Monad m] [LawfulMonad m] (f : β → α → m β) (b) (l l' : List α) :
+    (l ++ l').foldlM f b = l.foldlM f b >>= l'.foldlM f := by
+  induction l generalizing b <;> simp [*]
 
-theorem length_pos_of_mem {a : α} : ∀ {l : List α}, a ∈ l → 0 < length l
-  | _::_, _ => Nat.zero_lt_succ _
+@[simp] theorem foldrM_cons [Monad m] [LawfulMonad m] (a : α) (l) (f : α → β → m β) (b) :
+    (a :: l).foldrM f b = l.foldrM f b >>= f a := by
+  simp only [foldrM]
+  induction l <;> simp_all
 
-theorem exists_mem_of_length_pos : ∀ {l : List α}, 0 < length l → ∃ a, a ∈ l
-  | _::_, _ => ⟨_, .head ..⟩
+theorem foldl_eq_foldlM (f : β → α → β) (b) (l : List α) :
+    l.foldl f b = l.foldlM (m := Id) f b := by
+  induction l generalizing b <;> simp [*, foldl]
 
-theorem length_pos_iff_exists_mem {l : List α} : 0 < length l ↔ ∃ a, a ∈ l :=
-  ⟨exists_mem_of_length_pos, fun ⟨_, h⟩ => length_pos_of_mem h⟩
+theorem foldr_eq_foldrM (f : α → β → β) (b) (l : List α) :
+    l.foldr f b = l.foldrM (m := Id) f b := by
+  induction l <;> simp [*, foldr]
 
-theorem exists_cons_of_length_pos : ∀ {l : List α}, 0 < l.length → ∃ h t, l = h :: t
-  | _::_, _ => ⟨_, _, rfl⟩
+/-! ### foldl and foldr -/
 
-theorem length_pos_iff_exists_cons :
-    ∀ {l : List α}, 0 < l.length ↔ ∃ h t, l = h :: t :=
-  ⟨exists_cons_of_length_pos, fun ⟨_, _, eq⟩ => eq ▸ Nat.succ_pos _⟩
+@[simp] theorem foldrM_append [Monad m] [LawfulMonad m] (f : α → β → m β) (b) (l l' : List α) :
+    (l ++ l').foldrM f b = l'.foldrM f b >>= l.foldrM f := by
+  induction l <;> simp [*]
 
-theorem exists_cons_of_length_succ :
-    ∀ {l : List α}, l.length = n + 1 → ∃ h t, l = h :: t
-  | _::_, _ => ⟨_, _, rfl⟩
+@[simp] theorem foldl_append {β : Type _} (f : β → α → β) (b) (l l' : List α) :
+    (l ++ l').foldl f b = l'.foldl f (l.foldl f b) := by simp [foldl_eq_foldlM]
 
-theorem length_pos {l : List α} : 0 < length l ↔ l ≠ [] :=
-  Nat.pos_iff_ne_zero.trans (not_congr length_eq_zero)
+@[simp] theorem foldr_append (f : α → β → β) (b) (l l' : List α) :
+    (l ++ l').foldr f b = l.foldr f (l'.foldr f b) := by simp [foldr_eq_foldrM]
 
-theorem exists_mem_of_ne_nil (l : List α) (h : l ≠ []) : ∃ x, x ∈ l :=
-  exists_mem_of_length_pos (length_pos.2 h)
+@[simp] theorem foldr_self_append (l : List α) : l.foldr cons l' = l ++ l' := by
+  induction l <;> simp [*]
 
-theorem length_eq_one {l : List α} : length l = 1 ↔ ∃ a, l = [a] :=
-  ⟨fun h => match l, h with | [_], _ => ⟨_, rfl⟩, fun ⟨_, h⟩ => by simp [h]⟩
+theorem foldr_self (l : List α) : l.foldr cons [] = l := by simp
 
-/-! ### mem -/
+theorem foldl_map (f : β₁ → β₂) (g : α → β₂ → α) (l : List β₁) (init : α) :
+    (l.map f).foldl g init = l.foldl (fun x y => g x (f y)) init := by
+  induction l generalizing init <;> simp [*]
 
-theorem mem_nil_iff (a : α) : a ∈ ([] : List α) ↔ False := by simp
+theorem foldr_map (f : α₁ → α₂) (g : α₂ → β → β) (l : List α₁) (init : β) :
+    (l.map f).foldr g init = l.foldr (fun x y => g (f x) y) init := by
+  induction l generalizing init <;> simp [*]
 
-theorem mem_singleton_self (a : α) : a ∈ [a] := mem_cons_self _ _
+/-! ### lt -/
 
-theorem eq_of_mem_singleton : a ∈ [b] → a = b
-  | .head .. => rfl
+theorem lt_irrefl' [LT α] (lt_irrefl : ∀ x : α, ¬x < x) (l : List α) : ¬l < l := by
+  induction l with
+  | nil => nofun
+  | cons a l ih => intro
+    | .head _ _ h => exact lt_irrefl _ h
+    | .tail _ _ h => exact ih h
 
-@[simp 1100] theorem mem_singleton {a b : α} : a ∈ [b] ↔ a = b :=
-  ⟨eq_of_mem_singleton, (by simp [·])⟩
+theorem lt_trans' [LT α] [DecidableRel (@LT.lt α _)]
+    (lt_trans : ∀ {x y z : α}, x < y → y < z → x < z)
+    (le_trans : ∀ {x y z : α}, ¬x < y → ¬y < z → ¬x < z)
+    {l₁ l₂ l₃ : List α} (h₁ : l₁ < l₂) (h₂ : l₂ < l₃) : l₁ < l₃ := by
+  induction h₁ generalizing l₃ with
+  | nil => let _::_ := l₃; exact List.lt.nil ..
+  | @head a l₁ b l₂ ab =>
+    match h₂ with
+    | .head l₂ l₃ bc => exact List.lt.head _ _ (lt_trans ab bc)
+    | .tail _ cb ih =>
+      exact List.lt.head _ _ <| Decidable.by_contra (le_trans · cb ab)
+  | @tail a l₁ b l₂ ab ba h₁ ih2 =>
+    match h₂ with
+    | .head l₂ l₃ bc =>
+      exact List.lt.head _ _ <| Decidable.by_contra (le_trans ba · bc)
+    | .tail bc cb ih =>
+      exact List.lt.tail (le_trans ab bc) (le_trans cb ba) (ih2 ih)
 
-theorem mem_of_mem_cons_of_mem : ∀ {a b : α} {l : List α}, a ∈ b :: l → b ∈ l → a ∈ l
-  | _, _, _, .head .., h | _, _, _, .tail _ h, _ => h
+theorem lt_antisymm' [LT α]
+    (lt_antisymm : ∀ {x y : α}, ¬x < y → ¬y < x → x = y)
+    {l₁ l₂ : List α} (h₁ : ¬l₁ < l₂) (h₂ : ¬l₂ < l₁) : l₁ = l₂ := by
+  induction l₁ generalizing l₂ with
+  | nil =>
+    cases l₂ with
+    | nil => rfl
+    | cons b l₂ => cases h₁ (.nil ..)
+  | cons a l₁ ih =>
+    cases l₂ with
+    | nil => cases h₂ (.nil ..)
+    | cons b l₂ =>
+      have ab : ¬a < b := fun ab => h₁ (.head _ _ ab)
+      cases lt_antisymm ab (fun ba => h₂ (.head _ _ ba))
+      rw [ih (fun ll => h₁ (.tail ab ab ll)) (fun ll => h₂ (.tail ab ab ll))]
 
-theorem eq_or_ne_mem_of_mem {a b : α} {l : List α} (h' : a ∈ b :: l) : a = b ∨ (a ≠ b ∧ a ∈ l) :=
-  (Classical.em _).imp_right fun h => ⟨h, (mem_cons.1 h').resolve_left h⟩
 
-theorem ne_nil_of_mem {a : α} {l : List α} (h : a ∈ l) : l ≠ [] := by cases h <;> nofun
+/-! ### getD -/
+
+@[simp] theorem getD_eq_getElem? (l) (n) (a : α) : getD l n a = (l[n]?).getD a := by
+  simp [getD]
+
+@[deprecated getD_eq_getElem? (since := "2024-06-12")]
+theorem getD_eq_get? : ∀ l n (a : α), getD l n a = (get? l n).getD a := by simp
+
+/-! ### getLast -/
+
+theorem getLast_eq_get : ∀ (l : List α) (h : l ≠ []),
+    getLast l h = l.get ⟨l.length - 1, by
+      match l with
+      | [] => contradiction
+      | a :: l => exact Nat.le_refl _⟩
+  | [a], h => rfl
+  | a :: b :: l, h => by
+    simp [getLast, get, Nat.succ_sub_succ, getLast_eq_get]
+
+theorem getLast_cons' {a : α} {l : List α} : ∀ (h₁ : a :: l ≠ nil) (h₂ : l ≠ nil),
+  getLast (a :: l) h₁ = getLast l h₂ := by
+  induction l <;> intros; {contradiction}; rfl
+
+theorem getLast_eq_getLastD (a l h) : @getLast α (a::l) h = getLastD l a := by
+  cases l <;> rfl
+
+theorem getLastD_eq_getLast? (a l) : @getLastD α l a = (getLast? l).getD a := by
+  cases l <;> rfl
+
+@[simp] theorem getLast_singleton (a h) : @getLast α [a] h = a := rfl
+
+theorem getLast!_cons [Inhabited α] : @getLast! α _ (a::l) = getLastD l a := by
+  simp [getLast!, getLast_eq_getLastD]
+
+theorem getLast_mem : ∀ {l : List α} (h : l ≠ []), getLast l h ∈ l
+  | [], h => absurd rfl h
+  | [_], _ => .head ..
+  | _::a::l, _ => .tail _ <| getLast_mem (cons_ne_nil a l)
+
+theorem getLastD_mem_cons : ∀ (l : List α) (a : α), getLastD l a ∈ a::l
+  | [], _ => .head ..
+  | _::_, _ => .tail _ <| getLast_mem _
+
+theorem getElem_cons_length (x : α) (xs : List α) (n : Nat) (h : n = xs.length) :
+    (x :: xs)[n]'(by simp [h]) = (x :: xs).getLast (cons_ne_nil x xs) := by
+  rw [getLast_eq_get]; cases h; rfl
+
+@[deprecated getElem_cons_length (since := "2024-06-12")]
+theorem get_cons_length (x : α) (xs : List α) (n : Nat) (h : n = xs.length) :
+    (x :: xs).get ⟨n, by simp [h]⟩ = (x :: xs).getLast (cons_ne_nil x xs) := by
+  simp [getElem_cons_length, h]
+
+/-! ### getLast? -/
+
+theorem getLast?_cons : @getLast? α (a::l) = getLastD l a := by
+  simp [getLast?, getLast_eq_getLastD]
+
+@[simp] theorem getLast?_singleton (a : α) : getLast? [a] = a := rfl
+
+theorem getLast?_eq_getLast : ∀ l h, @getLast? α l = some (getLast l h)
+  | [], h => nomatch h rfl
+  | _::_, _ => rfl
+
+theorem getLast?_eq_get? : ∀ (l : List α), getLast? l = l.get? (l.length - 1)
+  | [] => rfl
+  | a::l => by rw [getLast?_eq_getLast (a::l) nofun, getLast_eq_get, get?_eq_get]
+
+@[simp] theorem getLast?_concat (l : List α) : getLast? (l ++ [a]) = some a := by
+  simp [getLast?_eq_get?, Nat.succ_sub_succ]
+
+@[simp] theorem getLastD_concat (a b l) : @getLastD α (l ++ [b]) a = b := by
+  rw [getLastD_eq_getLast?, getLast?_concat]; rfl
+
+/-! ### head -/
+
+theorem head!_of_head? [Inhabited α] : ∀ {l : List α}, head? l = some a → head! l = a
+  | _a::_l, rfl => rfl
+
+theorem head?_eq_head : ∀ l h, @head? α l = some (head l h)
+  | _::_, _ => rfl
+
+/-! ### tail -/
+
+@[simp] theorem tailD_eq_tail? (l l' : List α) : tailD l l' = (tail? l).getD l' := by
+  cases l <;> rfl
+
+/-! ### map -/
+
+@[simp] theorem length_map (as : List α) (f : α → β) : (as.map f).length = as.length := by
+  induction as with
+  | nil => simp [List.map]
+  | cons _ as ih => simp [List.map, ih]
+
+@[simp] theorem getElem?_map (f : α → β) : ∀ (l : List α) (n : Nat), (map f l)[n]? = Option.map f l[n]?
+  | [], _ => rfl
+  | _ :: _, 0 => by simp
+  | _ :: l, n+1 => by simp [getElem?_map f l n]
+
+@[deprecated getElem?_map (since := "2024-06-12")]
+theorem get?_map (f : α → β) : ∀ l n, (map f l).get? n = (l.get? n).map f
+  | [], _ => rfl
+  | _ :: _, 0 => rfl
+  | _ :: l, n+1 => get?_map f l n
+
+@[simp] theorem getElem_map (f : α → β) {l} {n : Nat} {h : n < (map f l).length} :
+    (map f l)[n] = f (l[n]'(length_map l f ▸ h)) :=
+  Option.some.inj <| by rw [← getElem?_eq_getElem, getElem?_map, getElem?_eq_getElem]; rfl
+
+@[deprecated getElem_map (since := "2024-06-12")]
+theorem get_map (f : α → β) {l n} :
+    get (map f l) n = f (get l ⟨n, length_map l f ▸ n.2⟩) := by
+  simp
+
+@[simp] theorem map_append (f : α → β) : ∀ l₁ l₂, map f (l₁ ++ l₂) = map f l₁ ++ map f l₂ := by
+  intro l₁; induction l₁ <;> intros <;> simp_all
+
+@[simp] theorem map_id (l : List α) : map id l = l := by induction l <;> simp_all
+
+@[simp] theorem map_id' (l : List α) : map (fun a => a) l = l := by induction l <;> simp_all
+
+@[simp] theorem mem_map {f : α → β} : ∀ {l : List α}, b ∈ l.map f ↔ ∃ a, a ∈ l ∧ f a = b
+  | [] => by simp
+  | _ :: l => by simp [mem_map (l := l), eq_comm (a := b)]
+
+theorem mem_map_of_mem (f : α → β) (h : a ∈ l) : f a ∈ map f l := mem_map.2 ⟨_, h, rfl⟩
+
+@[simp] theorem map_map (g : β → γ) (f : α → β) (l : List α) :
+  map g (map f l) = map (g ∘ f) l := by induction l <;> simp_all
+
+theorem map_singleton (f : α → β) (a : α) : map f [a] = [f a] := rfl
+
+theorem exists_of_mem_map (h : b ∈ map f l) : ∃ a, a ∈ l ∧ f a = b := mem_map.1 h
+
+theorem forall_mem_map_iff {f : α → β} {l : List α} {P : β → Prop} :
+    (∀ (i) (_ : i ∈ l.map f), P i) ↔ ∀ (j) (_ : j ∈ l), P (f j) := by
+  simp
+
+@[simp] theorem map_eq_nil {f : α → β} {l : List α} : map f l = [] ↔ l = [] := by
+  constructor <;> exact fun _ => match l with | [] => rfl
+
+/-! ### filter -/
+
+@[simp] theorem filter_cons_of_pos {p : α → Bool} {a : α} (l) (pa : p a) :
+    filter p (a :: l) = a :: filter p l := by rw [filter, pa]
+
+@[simp] theorem filter_cons_of_neg {p : α → Bool} {a : α} (l) (pa : ¬ p a) :
+    filter p (a :: l) = filter p l := by rw [filter, eq_false_of_ne_true pa]
+
+theorem filter_cons :
+    (x :: xs : List α).filter p = if p x then x :: (xs.filter p) else xs.filter p := by
+  split <;> simp [*]
+
+theorem mem_filter : x ∈ filter p as ↔ x ∈ as ∧ p x := by
+  induction as with
+  | nil => simp [filter]
+  | cons a as ih =>
+    by_cases h : p a
+    · simp_all [or_and_left]
+    · simp_all [or_and_right]
+
+theorem filter_eq_nil {l} : filter p l = [] ↔ ∀ a, a ∈ l → ¬p a := by
+  simp only [eq_nil_iff_forall_not_mem, mem_filter, not_and]
+
+@[simp] theorem filter_filter (q) : ∀ l, filter p (filter q l) = filter (fun a => p a ∧ q a) l
+  | [] => rfl
+  | a :: l => by by_cases hp : p a <;> by_cases hq : q a <;> simp [hp, hq, filter_filter _ l]
+
+theorem filter_map (f : β → α) (l : List β) : filter p (map f l) = map f (filter (p ∘ f) l) := by
+  induction l with
+  | nil => rfl
+  | cons a l IH => by_cases h : p (f a) <;> simp [*]
+
+@[deprecated filter_map (since := "2024-06-15")] abbrev map_filter := @filter_map
+
+@[simp] theorem filter_append {p : α → Bool} :
+    ∀ (l₁ l₂ : List α), filter p (l₁ ++ l₂) = filter p l₁ ++ filter p l₂
+  | [], l₂ => rfl
+  | a :: l₁, l₂ => by simp [filter]; split <;> simp [filter_append l₁]
+
+theorem filter_congr' {p q : α → Bool} :
+    ∀ {l : List α}, (∀ x ∈ l, p x ↔ q x) → filter p l = filter q l
+  | [], _ => rfl
+  | a :: l, h => by
+    rw [forall_mem_cons] at h; by_cases pa : p a
+    · simp [pa, h.1.1 pa, filter_congr' h.2]
+    · simp [pa, mt h.1.2 pa, filter_congr' h.2]
+
+/-! ### filterMap -/
+
+theorem filterMap_cons_none {f : α → Option β} (a : α) (l : List α) (h : f a = none) :
+    filterMap f (a :: l) = filterMap f l := by simp only [filterMap, h]
+
+theorem filterMap_cons_some (f : α → Option β) (a : α) (l : List α) {b : β} (h : f a = some b) :
+    filterMap f (a :: l) = b :: filterMap f l := by simp only [filterMap, h]
+
+@[simp]
+theorem filterMap_eq_map (f : α → β) : filterMap (some ∘ f) = map f := by
+  funext l; induction l <;> simp [*]
+
+@[simp] theorem filterMap_some (l : List α) : filterMap some l = l := by
+  erw [filterMap_eq_map, map_id]
+
+theorem filterMap_append {α β : Type _} (l l' : List α) (f : α → Option β) :
+    filterMap f (l ++ l') = filterMap f l ++ filterMap f l' := by
+  induction l <;> simp; split <;> simp [*]
+
+@[simp]
+theorem filterMap_eq_filter (p : α → Bool) :
+    filterMap (Option.guard (p ·)) = filter p := by
+  funext l
+  induction l with
+  | nil => rfl
+  | cons a l IH => by_cases pa : p a <;> simp [Option.guard, pa, ← IH]
+
+theorem filterMap_filterMap (f : α → Option β) (g : β → Option γ) (l : List α) :
+    filterMap g (filterMap f l) = filterMap (fun x => (f x).bind g) l := by
+  induction l with
+  | nil => rfl
+  | cons a l IH => cases h : f a <;> simp [*]
+
+theorem map_filterMap (f : α → Option β) (g : β → γ) (l : List α) :
+    map g (filterMap f l) = filterMap (fun x => (f x).map g) l := by
+  simp only [← filterMap_eq_map, filterMap_filterMap, Option.map_eq_bind]
+
+@[simp]
+theorem filterMap_map (f : α → β) (g : β → Option γ) (l : List α) :
+    filterMap g (map f l) = filterMap (g ∘ f) l := by
+  rw [← filterMap_eq_map, filterMap_filterMap]; rfl
+
+theorem filter_filterMap (f : α → Option β) (p : β → Bool) (l : List α) :
+    filter p (filterMap f l) = filterMap (fun x => (f x).filter p) l := by
+  rw [← filterMap_eq_filter, filterMap_filterMap]
+  congr; funext x; cases f x <;> simp [Option.filter, Option.guard]
+
+theorem filterMap_filter (p : α → Bool) (f : α → Option β) (l : List α) :
+    filterMap f (filter p l) = filterMap (fun x => if p x then f x else none) l := by
+  rw [← filterMap_eq_filter, filterMap_filterMap]
+  congr; funext x; by_cases h : p x <;> simp [Option.guard, h]
+
+theorem map_filterMap_some_eq_filter_map_is_some (f : α → Option β) (l : List α) :
+    (l.filterMap f).map some = (l.map f).filter fun b => b.isSome := by
+  induction l <;> simp; split <;> simp [*]
+
+@[simp] theorem mem_filterMap (f : α → Option β) (l : List α) {b : β} :
+    b ∈ filterMap f l ↔ ∃ a, a ∈ l ∧ f a = some b := by
+  induction l <;> simp; split <;> simp [*, eq_comm]
+
+@[simp] theorem filterMap_join (f : α → Option β) (L : List (List α)) :
+    filterMap f (join L) = join (map (filterMap f) L) := by
+  induction L <;> simp [*, filterMap_append]
+
+theorem map_filterMap_of_inv (f : α → Option β) (g : β → α) (H : ∀ x : α, (f x).map g = some x)
+    (l : List α) : map g (filterMap f l) = l := by simp only [map_filterMap, H, filterMap_some]
+
+/-! ### append -/
+
+theorem getElem?_append_right : ∀ {l₁ l₂ : List α} {n : Nat}, l₁.length ≤ n →
+  (l₁ ++ l₂)[n]? = l₂[n - l₁.length]?
+| [], _, n, _ => rfl
+| a :: l, _, n+1, h₁ => by
+  rw [cons_append]
+  simp [Nat.succ_sub_succ_eq_sub, getElem?_append_right (Nat.lt_succ.1 h₁)]
+
+@[deprecated getElem?_append_right (since := "2024-06-12")]
+theorem get?_append_right {l₁ l₂ : List α} {n : Nat} (h : l₁.length ≤ n) :
+    (l₁ ++ l₂).get? n = l₂.get? (n - l₁.length) := by
+  simp [getElem?_append_right, h]
+
+theorem getElem_append_right' {l₁ l₂ : List α} {n : Nat} (h₁ : l₁.length ≤ n) (h₂) :
+    (l₁ ++ l₂)[n]'h₂ =
+      l₂[n - l₁.length]'(by rw [length_append] at h₂; exact Nat.sub_lt_left_of_lt_add h₁ h₂) :=
+  Option.some.inj <| by rw [← getElem?_eq_getElem, ← getElem?_eq_getElem, getElem?_append_right h₁]
+
+@[deprecated (since := "2024-06-12")]
+theorem get_append_right_aux {l₁ l₂ : List α} {n : Nat}
+  (h₁ : l₁.length ≤ n) (h₂ : n < (l₁ ++ l₂).length) : n - l₁.length < l₂.length := by
+  rw [length_append] at h₂
+  exact Nat.sub_lt_left_of_lt_add h₁ h₂
+
+set_option linter.deprecated false in
+@[deprecated getElem_append_right' (since := "2024-06-12")]
+theorem get_append_right' {l₁ l₂ : List α} {n : Nat} (h₁ : l₁.length ≤ n) (h₂) :
+    (l₁ ++ l₂).get ⟨n, h₂⟩ = l₂.get ⟨n - l₁.length, get_append_right_aux h₁ h₂⟩ :=
+  Option.some.inj <| by rw [← get?_eq_get, ← get?_eq_get, get?_append_right h₁]
+
+theorem getElem_of_append {l : List α} (eq : l = l₁ ++ a :: l₂) (h : l₁.length = n) :
+    l[n]'(eq ▸ h ▸ by simp_arith) = a := Option.some.inj <| by
+  rw [← getElem?_eq_getElem, eq, getElem?_append_right (h ▸ Nat.le_refl _), h]
+  simp
+
+@[deprecated (since := "2024-06-12")]
+theorem get_of_append_proof {l : List α}
+    (eq : l = l₁ ++ a :: l₂) (h : l₁.length = n) : n < length l := eq ▸ h ▸ by simp_arith
+
+set_option linter.deprecated false in
+@[deprecated getElem_of_append (since := "2024-06-12")]
+theorem get_of_append {l : List α} (eq : l = l₁ ++ a :: l₂) (h : l₁.length = n) :
+    l.get ⟨n, get_of_append_proof eq h⟩ = a := Option.some.inj <| by
+  rw [← get?_eq_get, eq, get?_append_right (h ▸ Nat.le_refl _), h, Nat.sub_self]; rfl
 
 theorem append_of_mem {a : α} {l : List α} : a ∈ l → ∃ s t : List α, l = s ++ a :: t
   | .head l => ⟨[], l, rfl⟩
   | .tail b h => let ⟨s, t, h'⟩ := append_of_mem h; ⟨b::s, t, by rw [h', cons_append]⟩
 
-theorem elem_iff [BEq α] [LawfulBEq α] {a : α} {as : List α} :
-    elem a as = true ↔ a ∈ as := ⟨mem_of_elem_eq_true, elem_eq_true_of_mem⟩
+@[simp 1100] theorem singleton_append : [x] ++ l = x :: l := rfl
 
-@[simp] theorem elem_eq_mem [BEq α] [LawfulBEq α] (a : α) (as : List α) :
-    elem a as = decide (a ∈ as) := by rw [Bool.eq_iff_iff, elem_iff, decide_eq_true_iff]
+theorem append_inj :
+    ∀ {s₁ s₂ t₁ t₂ : List α}, s₁ ++ t₁ = s₂ ++ t₂ → length s₁ = length s₂ → s₁ = s₂ ∧ t₁ = t₂
+  | [], [], t₁, t₂, h, _ => ⟨rfl, h⟩
+  | a :: s₁, b :: s₂, t₁, t₂, h, hl => by
+    simp [append_inj (cons.inj h).2 (Nat.succ.inj hl)] at h ⊢; exact h
 
-theorem mem_of_ne_of_mem {a y : α} {l : List α} (h₁ : a ≠ y) (h₂ : a ∈ y :: l) : a ∈ l :=
-  Or.elim (mem_cons.mp h₂) (absurd · h₁) (·)
+theorem append_inj_right (h : s₁ ++ t₁ = s₂ ++ t₂) (hl : length s₁ = length s₂) : t₁ = t₂ :=
+  (append_inj h hl).right
 
-theorem ne_of_not_mem_cons {a b : α} {l : List α} : a ∉ b::l → a ≠ b := mt (· ▸ .head _)
+theorem append_inj_left (h : s₁ ++ t₁ = s₂ ++ t₂) (hl : length s₁ = length s₂) : s₁ = s₂ :=
+  (append_inj h hl).left
 
-theorem not_mem_of_not_mem_cons {a b : α} {l : List α} : a ∉ b::l → a ∉ l := mt (.tail _)
+theorem append_inj' (h : s₁ ++ t₁ = s₂ ++ t₂) (hl : length t₁ = length t₂) : s₁ = s₂ ∧ t₁ = t₂ :=
+  append_inj h <| @Nat.add_right_cancel _ (length t₁) _ <| by
+  let hap := congrArg length h; simp only [length_append, ← hl] at hap; exact hap
 
-theorem not_mem_cons_of_ne_of_not_mem {a y : α} {l : List α} : a ≠ y → a ∉ l → a ∉ y::l :=
-  mt ∘ mem_of_ne_of_mem
+theorem append_inj_right' (h : s₁ ++ t₁ = s₂ ++ t₂) (hl : length t₁ = length t₂) : t₁ = t₂ :=
+  (append_inj' h hl).right
 
-theorem ne_and_not_mem_of_not_mem_cons {a y : α} {l : List α} : a ∉ y::l → a ≠ y ∧ a ∉ l :=
-  fun p => ⟨ne_of_not_mem_cons p, not_mem_of_not_mem_cons p⟩
+theorem append_inj_left' (h : s₁ ++ t₁ = s₂ ++ t₂) (hl : length t₁ = length t₂) : s₁ = s₂ :=
+  (append_inj' h hl).left
 
-/-! ### drop -/
+theorem append_right_inj {t₁ t₂ : List α} (s) : s ++ t₁ = s ++ t₂ ↔ t₁ = t₂ :=
+  ⟨fun h => append_inj_right h rfl, congrArg _⟩
 
-theorem drop_add : ∀ (m n) (l : List α), drop (m + n) l = drop m (drop n l)
-  | _, 0, _ => rfl
-  | _, _ + 1, [] => drop_nil.symm
-  | m, n + 1, _ :: _ => drop_add m n _
+theorem append_left_inj {s₁ s₂ : List α} (t) : s₁ ++ t = s₂ ++ t ↔ s₁ = s₂ :=
+  ⟨fun h => append_inj_left' h rfl, congrArg (· ++ _)⟩
 
-@[simp]
-theorem drop_left : ∀ l₁ l₂ : List α, drop (length l₁) (l₁ ++ l₂) = l₂
+@[simp] theorem append_eq_nil : p ++ q = [] ↔ p = [] ∧ q = [] := by
+  cases p <;> simp
+
+@[simp] theorem getLast_append {a : α} : ∀ (l : List α) h, getLast (l ++ [a]) h = a
   | [], _ => rfl
-  | _ :: l₁, l₂ => drop_left l₁ l₂
+  | a::t, h => by
+    simp [getLast_cons' _ fun H => cons_ne_nil _ _ (append_eq_nil.1 H).2, getLast_append t]
 
-theorem drop_left' {l₁ l₂ : List α} {n} (h : length l₁ = n) : drop n (l₁ ++ l₂) = l₂ := by
-  rw [← h]; apply drop_left
+theorem getLast_concat : getLast (concat l a) h = a := by
+  simp [concat_eq_append, getLast_append]
 
-/-! ### isEmpty -/
+theorem getElem_append : ∀ {l₁ l₂ : List α} (n : Nat) (h : n < l₁.length),
+    (l₁ ++ l₂)[n]'(length_append .. ▸ Nat.lt_add_right _ h) = l₁[n]
+| a :: l, _, 0, h => rfl
+| a :: l, _, n+1, h => by simp only [get, cons_append]; apply getElem_append
 
-@[simp] theorem isEmpty_nil : ([] : List α).isEmpty = true := rfl
-@[simp] theorem isEmpty_cons : (x :: xs : List α).isEmpty = false := rfl
+@[deprecated getElem_append (since := "2024-06-12")]
+theorem get_append {l₁ l₂ : List α} (n : Nat) (h : n < l₁.length) :
+    (l₁ ++ l₂).get ⟨n, length_append .. ▸ Nat.lt_add_right _ h⟩ = l₁.get ⟨n, h⟩ := by
+  simp [getElem_append, h]
 
-/-! ### append -/
+@[deprecated getElem_append_left (since := "2024-06-12")]
+theorem get_append_left (as bs : List α) (h : i < as.length) {h'} : (as ++ bs).get ⟨i, h'⟩ = as.get ⟨i, h⟩ := by
+  simp [getElem_append_left, h, h']
+
+@[deprecated getElem_append_right (since := "2024-06-12")]
+theorem get_append_right (as bs : List α) (h : ¬ i < as.length) {h' h''} : (as ++ bs).get ⟨i, h'⟩ = bs.get ⟨i - as.length, h''⟩ := by
+  simp [getElem_append_right, h, h', h'']
+
+theorem getElem?_append {l₁ l₂ : List α} {n : Nat} (hn : n < l₁.length) :
+    (l₁ ++ l₂)[n]? = l₁[n]? := by
+  have hn' : n < (l₁ ++ l₂).length := Nat.lt_of_lt_of_le hn <|
+    length_append .. ▸ Nat.le_add_right ..
+  simp_all [getElem?_eq_getElem, getElem_append]
+
+@[deprecated (since := "2024-06-12")]
+theorem get?_append {l₁ l₂ : List α} {n : Nat} (hn : n < l₁.length) :
+    (l₁ ++ l₂).get? n = l₁.get? n := by
+  simp [getElem?_append hn]
 
 theorem append_eq_append : List.append l₁ l₂ = l₁ ++ l₂ := rfl
 
@@ -1034,40 +976,625 @@ theorem mem_append_right {a : α} (l₁ : List α) {l₂ : List α} (h : a ∈ l
 theorem mem_iff_append {a : α} {l : List α} : a ∈ l ↔ ∃ s t : List α, l = s ++ a :: t :=
   ⟨append_of_mem, fun ⟨s, t, e⟩ => e ▸ by simp⟩
 
-/-! ### concat -/
+theorem forall_mem_append {p : α → Prop} {l₁ l₂ : List α} :
+    (∀ (x) (_ : x ∈ l₁ ++ l₂), p x) ↔ (∀ (x) (_ : x ∈ l₁), p x) ∧ (∀ (x) (_ : x ∈ l₂), p x) := by
+  simp only [mem_append, or_imp, forall_and]
 
-theorem concat_nil (a : α) : concat [] a = [a] :=
-  rfl
+/-! ### join -/
 
-theorem concat_cons (a b : α) (l : List α) : concat (a :: l) b = a :: concat l b :=
-  rfl
+theorem mem_join : ∀ {L : List (List α)}, a ∈ L.join ↔ ∃ l, l ∈ L ∧ a ∈ l
+  | [] => by simp
+  | b :: l => by simp [mem_join, or_and_right, exists_or]
 
-theorem init_eq_of_concat_eq {a : α} {l₁ l₂ : List α} : concat l₁ a = concat l₂ a → l₁ = l₂ := by
+theorem exists_of_mem_join : a ∈ join L → ∃ l, l ∈ L ∧ a ∈ l := mem_join.1
+
+theorem mem_join_of_mem (lL : l ∈ L) (al : a ∈ l) : a ∈ join L := mem_join.2 ⟨l, lL, al⟩
+
+/-! ### bind -/
+
+@[simp] theorem append_bind xs ys (f : α → List β) :
+  List.bind (xs ++ ys) f = List.bind xs f ++ List.bind ys f := by
+  induction xs; {rfl}; simp_all [bind_cons, append_assoc]
+
+@[simp] theorem bind_id (l : List (List α)) : List.bind l id = l.join := by simp [List.bind]
+
+theorem mem_bind {f : α → List β} {b} {l : List α} : b ∈ l.bind f ↔ ∃ a, a ∈ l ∧ b ∈ f a := by
+  simp [List.bind, mem_join]
+  exact ⟨fun ⟨_, ⟨a, h₁, rfl⟩, h₂⟩ => ⟨a, h₁, h₂⟩, fun ⟨a, h₁, h₂⟩ => ⟨_, ⟨a, h₁, rfl⟩, h₂⟩⟩
+
+theorem exists_of_mem_bind {b : β} {l : List α} {f : α → List β} :
+    b ∈ List.bind l f → ∃ a, a ∈ l ∧ b ∈ f a := mem_bind.1
+
+theorem mem_bind_of_mem {b : β} {l : List α} {f : α → List β} {a} (al : a ∈ l) (h : b ∈ f a) :
+    b ∈ List.bind l f := mem_bind.2 ⟨a, al, h⟩
+
+theorem bind_map (f : β → γ) (g : α → List β) :
+    ∀ l : List α, map f (l.bind g) = l.bind fun a => (g a).map f
+  | [] => rfl
+  | a::l => by simp only [bind_cons, map_append, bind_map _ _ l]
+
+/-! ### replicate -/
+
+theorem replicate_succ (a : α) (n) : replicate (n+1) a = a :: replicate n a := rfl
+
+theorem mem_replicate {a b : α} : ∀ {n}, b ∈ replicate n a ↔ n ≠ 0 ∧ b = a
+  | 0 => by simp
+  | n+1 => by simp [mem_replicate, Nat.succ_ne_zero]
+
+theorem eq_of_mem_replicate {a b : α} {n} (h : b ∈ replicate n a) : b = a := (mem_replicate.1 h).2
+
+@[simp] theorem getElem_replicate (a : α) {n : Nat} {m} (h : m < (replicate n a).length) :
+    (replicate n a)[m] = a :=
+  eq_of_mem_replicate (get_mem _ _ _)
+
+@[deprecated getElem_replicate (since := "2024-06-12")]
+theorem get_replicate (a : α) {n : Nat} (m : Fin _) : (replicate n a).get m = a := by
   simp
 
-theorem last_eq_of_concat_eq {a b : α} {l : List α} : concat l a = concat l b → a = b := by
+theorem eq_replicate_of_mem {a : α} :
+    ∀ {l : List α}, (∀ (b) (_ : b ∈ l), b = a) → l = replicate l.length a
+  | [], _ => rfl
+  | b :: l, H => by
+    let ⟨rfl, H₂⟩ := forall_mem_cons (l := l).1 H
+    rw [length_cons, replicate, ← eq_replicate_of_mem H₂]
+
+theorem eq_replicate {a : α} {n} {l : List α} :
+    l = replicate n a ↔ length l = n ∧ ∀ (b) (_ : b ∈ l), b = a :=
+  ⟨fun h => h ▸ ⟨length_replicate .., fun _ => eq_of_mem_replicate⟩,
+   fun ⟨e, al⟩ => e ▸ eq_replicate_of_mem al⟩
+
+/-! ### reverse -/
+
+@[simp] theorem length_reverse (as : List α) : (as.reverse).length = as.length := by
+  induction as with
+  | nil => rfl
+  | cons a as ih => simp [ih]
+
+theorem getElem?_reverse' : ∀ {l : List α} (i j), i + j + 1 = length l →
+    l.reverse[i]? = l[j]?
+  | [], _, _, _ => rfl
+  | a::l, i, 0, h => by simp [Nat.succ.injEq] at h; simp [h, getElem?_append_right, Nat.succ.injEq]
+  | a::l, i, j+1, h => by
+    have := Nat.succ.inj h; simp at this ⊢
+    rw [getElem?_append, getElem?_reverse' _ _ this]
+    rw [length_reverse, ← this]; apply Nat.lt_add_of_pos_right (Nat.succ_pos _)
+
+@[deprecated getElem?_reverse' (since := "2024-06-12")]
+theorem get?_reverse' {l : List α} (i j) (h : i + j + 1 = length l) : get? l.reverse i = get? l j := by
+  simp [getElem?_reverse' _ _ h]
+
+theorem getElem?_reverse {l : List α} {i} (h : i < length l) :
+    l.reverse[i]? = l[l.length - 1 - i]? :=
+  getElem?_reverse' _ _ <| by
+    rw [Nat.add_sub_of_le (Nat.le_sub_one_of_lt h),
+      Nat.sub_add_cancel (Nat.lt_of_le_of_lt (Nat.zero_le _) h)]
+
+@[deprecated getElem?_reverse (since := "2024-06-12")]
+theorem get?_reverse {l : List α} {i} (h : i < length l) :
+    get? l.reverse i = get? l (l.length - 1 - i) := by
+  simp [getElem?_reverse h]
+
+theorem reverseAux_reverseAux_nil (as bs : List α) : reverseAux (reverseAux as bs) [] = reverseAux bs as := by
+  induction as generalizing bs with
+  | nil => rfl
+  | cons a as ih => simp [reverseAux, ih]
+
+@[simp] theorem reverse_reverse (as : List α) : as.reverse.reverse = as := by
+  simp only [reverse]; rw [reverseAux_reverseAux_nil]; rfl
+
+@[simp] theorem getLast?_reverse (l : List α) : l.reverse.getLast? = l.head? := by cases l <;> simp
+
+@[simp] theorem head?_reverse (l : List α) : l.reverse.head? = l.getLast? := by
+  rw [← getLast?_reverse, reverse_reverse]
+
+@[simp] theorem reverse_append (as bs : List α) : (as ++ bs).reverse = bs.reverse ++ as.reverse := by
+  induction as <;> simp_all
+
+theorem reverse_map (f : α → β) (l : List α) : (l.map f).reverse = l.reverse.map f := by
+  induction l <;> simp [*]
+
+@[simp] theorem reverse_eq_nil_iff {xs : List α} : xs.reverse = [] ↔ xs = [] := by
+  match xs with
+  | [] => simp
+  | x :: xs => simp
+
+@[simp] theorem mem_reverseAux {x : α} : ∀ {as bs}, x ∈ reverseAux as bs ↔ x ∈ as ∨ x ∈ bs
+  | [], _ => ⟨.inr, fun | .inr h => h⟩
+  | a :: _, _ => by rw [reverseAux, mem_cons, or_assoc, or_left_comm, mem_reverseAux, mem_cons]
+
+@[simp] theorem mem_reverse {x : α} {as : List α} : x ∈ reverse as ↔ x ∈ as := by simp [reverse]
+
+theorem reverseAux_eq (as bs : List α) : reverseAux as bs = reverse as ++ bs :=
+  reverseAux_eq_append ..
+
+@[simp] theorem foldrM_reverse [Monad m] (l : List α) (f : α → β → m β) (b) :
+    l.reverse.foldrM f b = l.foldlM (fun x y => f y x) b :=
+  (foldlM_reverse ..).symm.trans <| by simp
+
+@[simp] theorem foldl_reverse (l : List α) (f : β → α → β) (b) :
+    l.reverse.foldl f b = l.foldr (fun x y => f y x) b := by simp [foldl_eq_foldlM, foldr_eq_foldrM]
+
+@[simp] theorem foldr_reverse (l : List α) (f : α → β → β) (b) :
+    l.reverse.foldr f b = l.foldl (fun x y => f y x) b :=
+  (foldl_reverse ..).symm.trans <| by simp
+
+/-! ### elem -/
+
+@[simp] theorem elem_cons_self [BEq α] [LawfulBEq α] {a : α} : (a::as).elem a = true := by
+  simp [elem_cons]
+
+/-! ### contains -/
+
+@[simp] theorem contains_cons [BEq α] :
+    (a :: as : List α).contains x = (a == x || as.contains x) := by
+  simp only [contains, elem]
+  split <;> simp_all
+
+theorem contains_eq_any_beq [BEq α] (l : List α) (a : α) : l.contains a = l.any (· == a) := by
+  induction l with simp | cons b l => cases b == a <;> simp [*]
+
+/-! ### take and drop
+
+Further results on `List.take` and `List.drop`, which rely on stronger automation in `Nat`,
+are given in `Init.Data.List.TakeDrop`.
+-/
+
+@[simp] theorem take_append_drop : ∀ (n : Nat) (l : List α), take n l ++ drop n l = l
+  | 0, _ => rfl
+  | _+1, [] => rfl
+  | n+1, x :: xs => congrArg (cons x) <| take_append_drop n xs
+
+@[simp] theorem length_drop : ∀ (i : Nat) (l : List α), length (drop i l) = length l - i
+  | 0, _ => rfl
+  | succ i, [] => Eq.symm (Nat.zero_sub (succ i))
+  | succ i, x :: l => calc
+    length (drop (succ i) (x :: l)) = length l - i := length_drop i l
+    _ = succ (length l) - succ i := (Nat.succ_sub_succ_eq_sub (length l) i).symm
+
+theorem drop_length_le {l : List α} (h : l.length ≤ i) : drop i l = [] :=
+  length_eq_zero.1 (length_drop .. ▸ Nat.sub_eq_zero_of_le h)
+
+theorem take_length_le {l : List α} (h : l.length ≤ i) : take i l = l := by
+  have := take_append_drop i l
+  rw [drop_length_le h, append_nil] at this; exact this
+
+@[simp] theorem drop_length (l : List α) : drop l.length l = [] := drop_length_le (Nat.le_refl _)
+
+@[simp] theorem take_length (l : List α) : take l.length l = l := take_length_le (Nat.le_refl _)
+
+theorem take_concat_get (l : List α) (i : Nat) (h : i < l.length) :
+    (l.take i).concat l[i] = l.take (i+1) :=
+  Eq.symm <| (append_left_inj _).1 <| (take_append_drop (i+1) l).trans <| by
+    rw [concat_eq_append, append_assoc, singleton_append, get_drop_eq_drop, take_append_drop]
+
+theorem reverse_concat (l : List α) (a : α) : (l.concat a).reverse = a :: l.reverse := by
+  rw [concat_eq_append, reverse_append]; rfl
+
+abbrev take_succ_cons := @take_cons_succ
+
+theorem take_all_of_le {n} {l : List α} (h : length l ≤ n) : take n l = l :=
+  take_length_le h
+
+@[simp]
+theorem take_left : ∀ l₁ l₂ : List α, take (length l₁) (l₁ ++ l₂) = l₁
+  | [], _ => rfl
+  | a :: l₁, l₂ => congrArg (cons a) (take_left l₁ l₂)
+
+theorem take_left' {l₁ l₂ : List α} {n} (h : length l₁ = n) : take n (l₁ ++ l₂) = l₁ := by
+  rw [← h]; apply take_left
+
+theorem map_take (f : α → β) :
+    ∀ (L : List α) (i : Nat), (L.take i).map f = (L.map f).take i
+  | [], i => by simp
+  | _, 0 => by simp
+  | h :: t, n + 1 => by dsimp; rw [map_take f t n]
+
+theorem getElem?_take {l : List α} {n m : Nat} (h : m < n) : (l.take n)[m]? = l[m]? := by
+  induction n generalizing l m with
+  | zero =>
+    exact absurd h (Nat.not_lt_of_le m.zero_le)
+  | succ _ hn =>
+    cases l with
+    | nil => simp only [take_nil]
+    | cons hd tl =>
+      cases m
+      · simp
+      · simpa using hn (Nat.lt_of_succ_lt_succ h)
+
+@[deprecated getElem?_take (since := "2024-06-12")]
+theorem get?_take {l : List α} {n m : Nat} (h : m < n) : (l.take n).get? m = l.get? m := by
+  simp [getElem?_take, h]
+
+@[simp]
+theorem get?_take_of_succ {l : List α} {n : Nat} : (l.take (n + 1))[n]? = l[n]? :=
+  getElem?_take (Nat.lt_succ_self n)
+
+theorem take_succ {l : List α} {n : Nat} : l.take (n + 1) = l.take n ++ l[n]?.toList := by
+  induction l generalizing n with
+  | nil =>
+    simp only [take_nil, Option.toList, getElem?_nil, append_nil]
+  | cons hd tl hl =>
+    cases n
+    · simp only [take, Option.toList, getElem?_cons_zero, nil_append]
+    · simp only [take, hl, getElem?_cons_succ, cons_append]
+
+@[simp]
+theorem take_eq_nil_iff {l : List α} {k : Nat} : l.take k = [] ↔ l = [] ∨ k = 0 := by
+  cases l <;> cases k <;> simp [Nat.succ_ne_zero]
+
+theorem take_eq_nil_of_eq_nil : ∀ {as : List α} {i}, as = [] → as.take i = []
+  | _, _, rfl => take_nil
+
+theorem ne_nil_of_take_ne_nil {as : List α} {i : Nat} (h: as.take i ≠ []) : as ≠ [] :=
+  mt take_eq_nil_of_eq_nil h
+
+theorem dropLast_eq_take (l : List α) : l.dropLast = l.take l.length.pred := by
+  cases l with
+  | nil => simp [dropLast]
+  | cons x l =>
+    induction l generalizing x with
+    | nil => simp [dropLast]
+    | cons hd tl hl => simp [dropLast, hl]
+
+@[simp]
+theorem drop_eq_nil_iff_le {l : List α} {k : Nat} : l.drop k = [] ↔ l.length ≤ k := by
+  refine' ⟨fun h => _, drop_eq_nil_of_le⟩
+  induction k generalizing l with
+  | zero =>
+    simp only [drop] at h
+    simp [h]
+  | succ k hk =>
+    cases l
+    · simp
+    · simp only [drop] at h
+      simpa [Nat.succ_le_succ_iff] using hk h
+
+theorem drop_sizeOf_le [SizeOf α] (l : List α) (n : Nat) : sizeOf (l.drop n) ≤ sizeOf l := by
+  induction l generalizing n with
+  | nil => rw [drop_nil]; apply Nat.le_refl
+  | cons _ _ lih =>
+    induction n with
+    | zero => apply Nat.le_refl
+    | succ n =>
+      exact Trans.trans (lih _) (Nat.le_add_left _ _)
+
+@[simp] theorem drop_drop (n : Nat) : ∀ (m) (l : List α), drop n (drop m l) = drop (n + m) l
+  | m, [] => by simp
+  | 0, l => by simp
+  | m + 1, a :: l =>
+    calc
+      drop n (drop (m + 1) (a :: l)) = drop n (drop m l) := rfl
+      _ = drop (n + m) l := drop_drop n m l
+      _ = drop (n + (m + 1)) (a :: l) := rfl
+
+theorem take_drop : ∀ (m n : Nat) (l : List α), take n (drop m l) = drop m (take (m + n) l)
+  | 0, _, _ => by simp
+  | _, _, [] => by simp
+  | _+1, _, _ :: _ => by simpa [Nat.succ_add, take_succ_cons, drop_succ_cons] using take_drop ..
+
+theorem map_drop (f : α → β) :
+    ∀ (L : List α) (i : Nat), (L.drop i).map f = (L.map f).drop i
+  | [], i => by simp
+  | L, 0 => by simp
+  | h :: t, n + 1 => by
+    dsimp
+    rw [map_drop f t]
+
+@[simp]
+theorem getElem_cons_drop : ∀ (l : List α) (i : Nat) (h : i < l.length),
+    l[i] :: drop (i + 1) l = drop i l
+  | _::_, 0, _ => rfl
+  | _::_, i+1, _ => getElem_cons_drop _ i _
+
+@[deprecated getElem_cons_drop (since := "2024-06-12")]
+theorem get_cons_drop (l : List α) (i) : get l i :: drop (i + 1) l = drop i l := by
   simp
 
-theorem concat_ne_nil (a : α) (l : List α) : concat l a ≠ [] := by simp
+theorem drop_eq_getElem_cons {n} {l : List α} (h) : drop n l = l[n] :: drop (n + 1) l :=
+  (getElem_cons_drop _ n h).symm
 
-theorem concat_append (a : α) (l₁ l₂ : List α) : concat l₁ a ++ l₂ = l₁ ++ a :: l₂ := by simp
+@[deprecated drop_eq_getElem_cons (since := "2024-06-12")]
+theorem drop_eq_get_cons {n} {l : List α} (h) : drop n l = get l ⟨n, h⟩ :: drop (n + 1) l := by
+  simp [drop_eq_getElem_cons]
 
-theorem append_concat (a : α) (l₁ l₂ : List α) : l₁ ++ concat l₂ a = concat (l₁ ++ l₂) a := by simp
+theorem drop_eq_nil_of_eq_nil : ∀ {as : List α} {i}, as = [] → as.drop i = []
+  | _, _, rfl => drop_nil
 
-/-! ### map -/
+theorem ne_nil_of_drop_ne_nil {as : List α} {i : Nat} (h: as.drop i ≠ []) : as ≠ [] :=
+  mt drop_eq_nil_of_eq_nil h
 
-theorem map_singleton (f : α → β) (a : α) : map f [a] = [f a] := rfl
+@[deprecated drop_drop (since := "2024-06-15")]
+theorem drop_add (m n) (l : List α) : drop (m + n) l = drop m (drop n l) := by
+  simp [drop_drop]
 
-theorem exists_of_mem_map (h : b ∈ map f l) : ∃ a, a ∈ l ∧ f a = b := mem_map.1 h
+@[simp]
+theorem drop_left : ∀ l₁ l₂ : List α, drop (length l₁) (l₁ ++ l₂) = l₂
+  | [], _ => rfl
+  | _ :: l₁, l₂ => drop_left l₁ l₂
 
-theorem forall_mem_map_iff {f : α → β} {l : List α} {P : β → Prop} :
-    (∀ (i) (_ : i ∈ l.map f), P i) ↔ ∀ (j) (_ : j ∈ l), P (f j) := by
+theorem drop_left' {l₁ l₂ : List α} {n} (h : length l₁ = n) : drop n (l₁ ++ l₂) = l₂ := by
+  rw [← h]; apply drop_left
+
+/-! ### takeWhile and dropWhile -/
+
+theorem dropWhile_cons :
+    (x :: xs : List α).dropWhile p = if p x then xs.dropWhile p else x :: xs := by
+  split <;> simp_all [dropWhile]
+
+@[simp] theorem takeWhile_append_dropWhile (p : α → Bool) :
+    ∀ (l : List α), takeWhile p l ++ dropWhile p l = l
+  | [] => rfl
+  | x :: xs => by simp [takeWhile, dropWhile]; cases p x <;> simp [takeWhile_append_dropWhile p xs]
+
+theorem dropWhile_append {xs ys : List α} :
+    (xs ++ ys).dropWhile p =
+      if (xs.dropWhile p).isEmpty then ys.dropWhile p else xs.dropWhile p ++ ys := by
+  induction xs with
+  | nil => simp
+  | cons h t ih =>
+    simp only [cons_append, dropWhile_cons]
+    split <;> simp_all
+
+/-! ### partition -/
+
+@[simp] theorem partition_eq_filter_filter (p : α → Bool) (l : List α) :
+    partition p l = (filter p l, filter (not ∘ p) l) := by simp [partition, aux] where
+  aux : ∀ l {as bs}, partition.loop p l (as, bs) =
+    (as.reverse ++ filter p l, bs.reverse ++ filter (not ∘ p) l)
+  | [] => by simp [partition.loop, filter]
+  | a :: l => by cases pa : p a <;> simp [partition.loop, pa, aux, filter, append_assoc]
+
+/-! ### dropLast
+
+`dropLast` is the specification for `Array.pop`, so theorems about `List.dropLast`
+are often used for theorems about `Array.pop`.
+-/
+
+@[simp] theorem length_dropLast : ∀ (xs : List α), xs.dropLast.length = xs.length - 1
+  | [] => rfl
+  | x::xs => by simp
+
+@[simp] theorem getElem_dropLast : ∀ (xs : List α) (i : Nat) (h : i < xs.dropLast.length),
+    xs.dropLast[i] = xs[i]'(Nat.lt_of_lt_of_le h (length_dropLast .. ▸ Nat.pred_le _))
+  | _::_::_, 0, _ => rfl
+  | _::_::_, i+1, _ => getElem_dropLast _ i _
+
+@[deprecated getElem_dropLast (since := "2024-06-12")]
+theorem get_dropLast (xs : List α) (i : Fin xs.dropLast.length) :
+    xs.dropLast.get i = xs.get ⟨i, Nat.lt_of_lt_of_le i.isLt (length_dropLast .. ▸ Nat.pred_le _)⟩ := by
   simp
 
-@[simp] theorem map_eq_nil {f : α → β} {l : List α} : map f l = [] ↔ l = [] := by
-  constructor <;> exact fun _ => match l with | [] => rfl
+theorem dropLast_cons_of_ne_nil {α : Type u} {x : α}
+    {l : List α} (h : l ≠ []) : (x :: l).dropLast = x :: l.dropLast := by
+  simp [dropLast, h]
+
+@[simp] theorem dropLast_append_of_ne_nil {α : Type u} {l : List α} :
+    ∀ (l' : List α) (_ : l ≠ []), (l' ++ l).dropLast = l' ++ l.dropLast
+  | [], _ => by simp only [nil_append]
+  | a :: l', h => by
+    rw [cons_append, dropLast, dropLast_append_of_ne_nil l' h, cons_append]
+    simp [h]
+
+theorem dropLast_append_cons : dropLast (l₁ ++ b::l₂) = l₁ ++ dropLast (b::l₂) := by
+  simp only [ne_eq, not_false_eq_true, dropLast_append_of_ne_nil]
+
+@[simp 1100] theorem dropLast_concat : dropLast (l₁ ++ [b]) = l₁ := by simp
+
+/-! ### isPrefixOf -/
+
+@[simp] theorem isPrefixOf_cons₂_self [BEq α] [LawfulBEq α] {a : α} :
+    isPrefixOf (a::as) (a::bs) = isPrefixOf as bs := by simp [isPrefixOf_cons₂]
+
+/-! ### replace -/
+
+@[simp] theorem replace_cons_self [BEq α] [LawfulBEq α] {a : α} : (a::as).replace a b = b::as := by
+  simp [replace_cons]
+
+/-! ### insert -/
+
+section insert
+variable [BEq α] [LawfulBEq α]
+
+@[simp] theorem insert_of_mem {l : List α} (h : a ∈ l) : l.insert a = l := by
+  simp [List.insert, h]
+
+@[simp] theorem insert_of_not_mem {l : List α} (h : a ∉ l) : l.insert a = a :: l := by
+  simp [List.insert, h]
+
+@[simp] theorem mem_insert_iff {l : List α} : a ∈ l.insert b ↔ a = b ∨ a ∈ l := by
+  if h : b ∈ l then
+    rw [insert_of_mem h]
+    constructor; {apply Or.inr}
+    intro
+    | Or.inl h' => rw [h']; exact h
+    | Or.inr h' => exact h'
+  else rw [insert_of_not_mem h, mem_cons]
+
+@[simp 1100] theorem mem_insert_self (a : α) (l : List α) : a ∈ l.insert a :=
+  mem_insert_iff.2 (Or.inl rfl)
+
+theorem mem_insert_of_mem {l : List α} (h : a ∈ l) : a ∈ l.insert b :=
+  mem_insert_iff.2 (Or.inr h)
+
+theorem eq_or_mem_of_mem_insert {l : List α} (h : a ∈ l.insert b) : a = b ∨ a ∈ l :=
+  mem_insert_iff.1 h
+
+@[simp] theorem length_insert_of_mem {l : List α} (h : a ∈ l) :
+    length (l.insert a) = length l := by rw [insert_of_mem h]
+
+@[simp] theorem length_insert_of_not_mem {l : List α} (h : a ∉ l) :
+    length (l.insert a) = length l + 1 := by rw [insert_of_not_mem h]; rfl
+
+end insert
+
+/-! ### erase -/
+
+section erase
+variable [BEq α]
+
+@[simp] theorem erase_cons_head [LawfulBEq α] (a : α) (l : List α) : (a :: l).erase a = l := by
+  simp [erase_cons]
+
+@[simp] theorem erase_cons_tail {a b : α} (l : List α) (h : ¬(b == a)) :
+    (b :: l).erase a = b :: l.erase a := by simp only [erase_cons, if_neg h]
+
+theorem erase_of_not_mem [LawfulBEq α] {a : α} : ∀ {l : List α}, a ∉ l → l.erase a = l
+  | [], _ => rfl
+  | b :: l, h => by
+    rw [mem_cons, not_or] at h
+    simp only [erase_cons, if_neg, erase_of_not_mem h.2, beq_iff_eq, Ne.symm h.1, not_false_eq_true]
+
+end erase
+
+/-! ### find? -/
+
+theorem find?_cons_of_pos (l) (h : p a) : find? p (a :: l) = some a :=
+  by simp [find?, h]
+
+theorem find?_cons_of_neg (l) (h : ¬p a) : find? p (a :: l) = find? p l :=
+  by simp [find?, h]
+
+theorem find?_eq_none : find? p l = none ↔ ∀ x ∈ l, ¬ p x := by
+  induction l <;> simp [find?_cons]; split <;> simp [*]
+
+theorem find?_some : ∀ {l}, find? p l = some a → p a
+  | b :: l, H => by
+    by_cases h : p b <;> simp [find?, h] at H
+    · exact H ▸ h
+    · exact find?_some H
+
+@[simp] theorem mem_of_find?_eq_some : ∀ {l}, find? p l = some a → a ∈ l
+  | b :: l, H => by
+    by_cases h : p b <;> simp [find?, h] at H
+    · exact H ▸ .head _
+    · exact .tail _ (mem_of_find?_eq_some H)
+
+/-! ### findSome? -/
+
+theorem exists_of_findSome?_eq_some {l : List α} {f : α → Option β} (w : l.findSome? f = some b) :
+    ∃ a, a ∈ l ∧ f a = b := by
+  induction l with
+  | nil => simp_all
+  | cons h l ih =>
+    simp_all only [findSome?_cons, mem_cons, exists_eq_or_imp]
+    split at w <;> simp_all
+
+/-! ### lookup -/
+
+@[simp] theorem lookup_cons_self [BEq α] [LawfulBEq α] {k : α} : ((k,b)::es).lookup k = some b := by
+  simp [lookup_cons]
+
+/-! ### any / all -/
+
+@[simp] theorem any_eq_true {l : List α} : l.any p ↔ ∃ x, x ∈ l ∧ p x := by induction l <;> simp [*]
+
+@[simp] theorem all_eq_true {l : List α} : l.all p ↔ ∀ x, x ∈ l →  p x := by induction l <;> simp [*]
+
+theorem not_any_eq_all_not (l : List α) (p : α → Bool) : (!l.any p) = l.all fun a => !p a := by
+  induction l with simp | cons _ _ ih => rw [ih]
+
+theorem not_all_eq_any_not (l : List α) (p : α → Bool) : (!l.all p) = l.any fun a => !p a := by
+  induction l with simp | cons _ _ ih => rw [ih]
+
+theorem and_any_distrib_left (l : List α) (p : α → Bool) (q : Bool) :
+    (q && l.any p) = l.any fun a => q && p a := by
+  induction l with simp | cons _ _ ih => rw [Bool.and_or_distrib_left, ih]
+
+theorem and_any_distrib_right (l : List α) (p : α → Bool) (q : Bool) :
+    (l.any p && q) = l.any fun a => p a && q := by
+  induction l with simp | cons _ _ ih => rw [Bool.and_or_distrib_right, ih]
+
+theorem or_all_distrib_left (l : List α) (p : α → Bool) (q : Bool) :
+    (q || l.all p) = l.all fun a => q || p a := by
+  induction l with simp | cons _ _ ih => rw [Bool.or_and_distrib_left, ih]
+
+theorem or_all_distrib_right (l : List α) (p : α → Bool) (q : Bool) :
+    (l.all p || q) = l.all fun a => p a || q := by
+  induction l with simp | cons _ _ ih => rw [Bool.or_and_distrib_right, ih]
+
+theorem any_eq_not_all_not (l : List α) (p : α → Bool) : l.any p = !l.all (!p .) := by
+  simp only [not_all_eq_any_not, Bool.not_not]
+
+theorem all_eq_not_any_not (l : List α) (p : α → Bool) : l.all p = !l.any (!p .) := by
+  simp only [not_any_eq_all_not, Bool.not_not]
+
+/-! ### zip -/
+
+theorem zip_map (f : α → γ) (g : β → δ) :
+    ∀ (l₁ : List α) (l₂ : List β), zip (l₁.map f) (l₂.map g) = (zip l₁ l₂).map (Prod.map f g)
+  | [], l₂ => rfl
+  | l₁, [] => by simp only [map, zip_nil_right]
+  | a :: l₁, b :: l₂ => by
+    simp only [map, zip_cons_cons, zip_map, Prod.map]; constructor
+
+theorem zip_map_left (f : α → γ) (l₁ : List α) (l₂ : List β) :
+    zip (l₁.map f) l₂ = (zip l₁ l₂).map (Prod.map f id) := by rw [← zip_map, map_id]
+
+theorem zip_map_right (f : β → γ) (l₁ : List α) (l₂ : List β) :
+    zip l₁ (l₂.map f) = (zip l₁ l₂).map (Prod.map id f) := by rw [← zip_map, map_id]
+
+theorem zip_append :
+    ∀ {l₁ r₁ : List α} {l₂ r₂ : List β} (_h : length l₁ = length l₂),
+      zip (l₁ ++ r₁) (l₂ ++ r₂) = zip l₁ l₂ ++ zip r₁ r₂
+  | [], r₁, l₂, r₂, h => by simp only [eq_nil_of_length_eq_zero h.symm]; rfl
+  | l₁, r₁, [], r₂, h => by simp only [eq_nil_of_length_eq_zero h]; rfl
+  | a :: l₁, r₁, b :: l₂, r₂, h => by
+    simp only [cons_append, zip_cons_cons, zip_append (Nat.succ.inj h)]
+
+theorem zip_map' (f : α → β) (g : α → γ) :
+    ∀ l : List α, zip (l.map f) (l.map g) = l.map fun a => (f a, g a)
+  | [] => rfl
+  | a :: l => by simp only [map, zip_cons_cons, zip_map']
+
+theorem of_mem_zip {a b} : ∀ {l₁ : List α} {l₂ : List β}, (a, b) ∈ zip l₁ l₂ → a ∈ l₁ ∧ b ∈ l₂
+  | _ :: l₁, _ :: l₂, h => by
+    cases h
+    case head => simp
+    case tail h =>
+    · have := of_mem_zip h
+      exact ⟨Mem.tail _ this.1, Mem.tail _ this.2⟩
+
+theorem map_fst_zip :
+    ∀ (l₁ : List α) (l₂ : List β), l₁.length ≤ l₂.length → map Prod.fst (zip l₁ l₂) = l₁
+  | [], bs, _ => rfl
+  | _ :: as, _ :: bs, h => by
+    simp [Nat.succ_le_succ_iff] at h
+    show _ :: map Prod.fst (zip as bs) = _ :: as
+    rw [map_fst_zip as bs h]
+  | a :: as, [], h => by simp at h
+
+theorem map_snd_zip :
+    ∀ (l₁ : List α) (l₂ : List β), l₂.length ≤ l₁.length → map Prod.snd (zip l₁ l₂) = l₂
+  | _, [], _ => by
+    rw [zip_nil_right]
+    rfl
+  | [], b :: bs, h => by simp at h
+  | a :: as, b :: bs, h => by
+    simp [Nat.succ_le_succ_iff] at h
+    show _ :: map Prod.snd (zip as bs) = _ :: bs
+    rw [map_snd_zip as bs h]
 
 /-! ### zipWith -/
+
+theorem getElem?_zipWith {f : α → β → γ} {i : Nat} :
+    (List.zipWith f as bs)[i]? = match as[i]?, bs[i]? with
+      | some a, some b => some (f a b) | _, _ => none := by
+  induction as generalizing bs i with
+  | nil => cases bs with
+    | nil => simp
+    | cons b bs => simp
+  | cons a as aih => cases bs with
+    | nil => simp
+    | cons b bs => cases i <;> simp_all
+
+@[deprecated getElem?_zipWith (since := "2024-06-12")]
+theorem get?_zipWith {f : α → β → γ} :
+    (List.zipWith f as bs).get? i = match as.get? i, bs.get? i with
+      | some a, some b => some (f a b) | _, _ => none := by
+  simp [getElem?_zipWith]
+
+set_option linter.deprecated false in
+@[deprecated getElem?_zipWith (since := "2024-06-07")] abbrev zipWith_get? := @get?_zipWith
 
 @[simp]
 theorem zipWith_map {μ} (f : γ → δ → μ) (g : α → γ) (h : β → δ) (l₁ : List α) (l₂ : List β) :
@@ -1137,687 +1664,111 @@ theorem zipWith_append (f : α → β → γ) (l la : List α) (l' lb : List β)
       simp only [length_cons, Nat.succ.injEq] at h
       simp [ih _ h]
 
-/-! ### zip -/
-
-theorem zip_map (f : α → γ) (g : β → δ) :
-    ∀ (l₁ : List α) (l₂ : List β), zip (l₁.map f) (l₂.map g) = (zip l₁ l₂).map (Prod.map f g)
-  | [], l₂ => rfl
-  | l₁, [] => by simp only [map, zip_nil_right]
-  | a :: l₁, b :: l₂ => by
-    simp only [map, zip_cons_cons, zip_map, Prod.map]; constructor
-
-theorem zip_map_left (f : α → γ) (l₁ : List α) (l₂ : List β) :
-    zip (l₁.map f) l₂ = (zip l₁ l₂).map (Prod.map f id) := by rw [← zip_map, map_id]
-
-theorem zip_map_right (f : β → γ) (l₁ : List α) (l₂ : List β) :
-    zip l₁ (l₂.map f) = (zip l₁ l₂).map (Prod.map id f) := by rw [← zip_map, map_id]
-
-theorem zip_append :
-    ∀ {l₁ r₁ : List α} {l₂ r₂ : List β} (_h : length l₁ = length l₂),
-      zip (l₁ ++ r₁) (l₂ ++ r₂) = zip l₁ l₂ ++ zip r₁ r₂
-  | [], r₁, l₂, r₂, h => by simp only [eq_nil_of_length_eq_zero h.symm]; rfl
-  | l₁, r₁, [], r₂, h => by simp only [eq_nil_of_length_eq_zero h]; rfl
-  | a :: l₁, r₁, b :: l₂, r₂, h => by
-    simp only [cons_append, zip_cons_cons, zip_append (Nat.succ.inj h)]
-
-theorem zip_map' (f : α → β) (g : α → γ) :
-    ∀ l : List α, zip (l.map f) (l.map g) = l.map fun a => (f a, g a)
-  | [] => rfl
-  | a :: l => by simp only [map, zip_cons_cons, zip_map']
-
-theorem of_mem_zip {a b} : ∀ {l₁ : List α} {l₂ : List β}, (a, b) ∈ zip l₁ l₂ → a ∈ l₁ ∧ b ∈ l₂
-  | _ :: l₁, _ :: l₂, h => by
-    cases h
-    case head => simp
-    case tail h =>
-    · have := of_mem_zip h
-      exact ⟨Mem.tail _ this.1, Mem.tail _ this.2⟩
-
-theorem map_fst_zip :
-    ∀ (l₁ : List α) (l₂ : List β), l₁.length ≤ l₂.length → map Prod.fst (zip l₁ l₂) = l₁
-  | [], bs, _ => rfl
-  | _ :: as, _ :: bs, h => by
-    simp [Nat.succ_le_succ_iff] at h
-    show _ :: map Prod.fst (zip as bs) = _ :: as
-    rw [map_fst_zip as bs h]
-  | a :: as, [], h => by simp at h
-
-theorem map_snd_zip :
-    ∀ (l₁ : List α) (l₂ : List β), l₂.length ≤ l₁.length → map Prod.snd (zip l₁ l₂) = l₂
-  | _, [], _ => by
-    rw [zip_nil_right]
-    rfl
-  | [], b :: bs, h => by simp at h
-  | a :: as, b :: bs, h => by
-    simp [Nat.succ_le_succ_iff] at h
-    show _ :: map Prod.snd (zip as bs) = _ :: bs
-    rw [map_snd_zip as bs h]
-
-/-! ### join -/
-
-theorem mem_join : ∀ {L : List (List α)}, a ∈ L.join ↔ ∃ l, l ∈ L ∧ a ∈ l
-  | [] => by simp
-  | b :: l => by simp [mem_join, or_and_right, exists_or]
-
-theorem exists_of_mem_join : a ∈ join L → ∃ l, l ∈ L ∧ a ∈ l := mem_join.1
-
-theorem mem_join_of_mem (lL : l ∈ L) (al : a ∈ l) : a ∈ join L := mem_join.2 ⟨l, lL, al⟩
-
-/-! ### bind -/
-
-theorem mem_bind {f : α → List β} {b} {l : List α} : b ∈ l.bind f ↔ ∃ a, a ∈ l ∧ b ∈ f a := by
-  simp [List.bind, mem_join]
-  exact ⟨fun ⟨_, ⟨a, h₁, rfl⟩, h₂⟩ => ⟨a, h₁, h₂⟩, fun ⟨a, h₁, h₂⟩ => ⟨_, ⟨a, h₁, rfl⟩, h₂⟩⟩
-
-theorem exists_of_mem_bind {b : β} {l : List α} {f : α → List β} :
-    b ∈ List.bind l f → ∃ a, a ∈ l ∧ b ∈ f a := mem_bind.1
-
-theorem mem_bind_of_mem {b : β} {l : List α} {f : α → List β} {a} (al : a ∈ l) (h : b ∈ f a) :
-    b ∈ List.bind l f := mem_bind.2 ⟨a, al, h⟩
-
-theorem bind_map (f : β → γ) (g : α → List β) :
-    ∀ l : List α, map f (l.bind g) = l.bind fun a => (g a).map f
-  | [] => rfl
-  | a::l => by simp only [cons_bind, map_append, bind_map _ _ l]
-
-/-! ### set-theoretic notation of Lists -/
-
-@[simp] theorem empty_eq : (∅ : List α) = [] := rfl
-
-/-! ### bounded quantifiers over Lists -/
-
-theorem exists_mem_nil (p : α → Prop) : ¬ (∃ x, ∃ _ : x ∈ @nil α, p x) := nofun
-
-theorem forall_mem_nil (p : α → Prop) : ∀ (x) (_ : x ∈ @nil α), p x := nofun
-
-theorem exists_mem_cons {p : α → Prop} {a : α} {l : List α} :
-    (∃ x, ∃ _ : x ∈ a :: l, p x) ↔ p a ∨ ∃ x, ∃ _ : x ∈ l, p x := by simp
-
-theorem forall_mem_singleton {p : α → Prop} {a : α} : (∀ (x) (_ : x ∈ [a]), p x) ↔ p a := by
-  simp only [mem_singleton, forall_eq]
-
-theorem forall_mem_append {p : α → Prop} {l₁ l₂ : List α} :
-    (∀ (x) (_ : x ∈ l₁ ++ l₂), p x) ↔ (∀ (x) (_ : x ∈ l₁), p x) ∧ (∀ (x) (_ : x ∈ l₂), p x) := by
-  simp only [mem_append, or_imp, forall_and]
-
-/-! ### replicate -/
-
-theorem replicate_succ (a : α) (n) : replicate (n+1) a = a :: replicate n a := rfl
-
-theorem mem_replicate {a b : α} : ∀ {n}, b ∈ replicate n a ↔ n ≠ 0 ∧ b = a
-  | 0 => by simp
-  | n+1 => by simp [mem_replicate, Nat.succ_ne_zero]
-
-theorem eq_of_mem_replicate {a b : α} {n} (h : b ∈ replicate n a) : b = a := (mem_replicate.1 h).2
-
-theorem eq_replicate_of_mem {a : α} :
-    ∀ {l : List α}, (∀ (b) (_ : b ∈ l), b = a) → l = replicate l.length a
-  | [], _ => rfl
-  | b :: l, H => by
-    let ⟨rfl, H₂⟩ := forall_mem_cons (l := l).1 H
-    rw [length_cons, replicate, ← eq_replicate_of_mem H₂]
-
-theorem eq_replicate {a : α} {n} {l : List α} :
-    l = replicate n a ↔ length l = n ∧ ∀ (b) (_ : b ∈ l), b = a :=
-  ⟨fun h => h ▸ ⟨length_replicate .., fun _ => eq_of_mem_replicate⟩,
-   fun ⟨e, al⟩ => e ▸ eq_replicate_of_mem al⟩
-
-/-! ### getLast -/
-
-theorem getLast_cons' {a : α} {l : List α} : ∀ (h₁ : a :: l ≠ nil) (h₂ : l ≠ nil),
-  getLast (a :: l) h₁ = getLast l h₂ := by
-  induction l <;> intros; {contradiction}; rfl
-
-@[simp] theorem getLast_append {a : α} : ∀ (l : List α) h, getLast (l ++ [a]) h = a
-  | [], _ => rfl
-  | a::t, h => by
-    simp [getLast_cons' _ fun H => cons_ne_nil _ _ (append_eq_nil.1 H).2, getLast_append t]
-
-theorem getLast_concat : (h : concat l a ≠ []) → getLast (concat l a) h = a :=
-  concat_eq_append .. ▸ getLast_append _
-
-theorem eq_nil_or_concat : ∀ l : List α, l = [] ∨ ∃ L b, l = L ++ [b]
-  | [] => .inl rfl
-  | a::l => match l, eq_nil_or_concat l with
-    | _, .inl rfl => .inr ⟨[], a, rfl⟩
-    | _, .inr ⟨L, b, rfl⟩ => .inr ⟨a::L, b, rfl⟩
-
-/-! ### head -/
-
-theorem head!_of_head? [Inhabited α] : ∀ {l : List α}, head? l = some a → head! l = a
-  | _a::_l, rfl => rfl
-
-theorem head?_eq_head : ∀ l h, @head? α l = some (head l h)
-  | _::_, _ => rfl
-
-/-! ### tail -/
-
-@[simp] theorem tailD_eq_tail? (l l' : List α) : tailD l l' = (tail? l).getD l' := by
-  cases l <;> rfl
-
-/-! ### getLast -/
-
-@[simp] theorem getLastD_nil (a) : @getLastD α [] a = a := rfl
-@[simp] theorem getLastD_cons (a b l) : @getLastD α (b::l) a = getLastD l b := by cases l <;> rfl
-
-theorem getLast_eq_getLastD (a l h) : @getLast α (a::l) h = getLastD l a := by
-  cases l <;> rfl
-
-theorem getLastD_eq_getLast? (a l) : @getLastD α l a = (getLast? l).getD a := by
-  cases l <;> rfl
-
-@[simp] theorem getLast_singleton (a h) : @getLast α [a] h = a := rfl
-
-theorem getLast!_cons [Inhabited α] : @getLast! α _ (a::l) = getLastD l a := by
-  simp [getLast!, getLast_eq_getLastD]
-
-theorem getLast?_cons : @getLast? α (a::l) = getLastD l a := by
-  simp [getLast?, getLast_eq_getLastD]
-
-@[simp] theorem getLast?_singleton (a : α) : getLast? [a] = a := rfl
-
-theorem getLast_mem : ∀ {l : List α} (h : l ≠ []), getLast l h ∈ l
-  | [], h => absurd rfl h
-  | [_], _ => .head ..
-  | _::a::l, _ => .tail _ <| getLast_mem (cons_ne_nil a l)
-
-theorem getLastD_mem_cons : ∀ (l : List α) (a : α), getLastD l a ∈ a::l
-  | [], _ => .head ..
-  | _::_, _ => .tail _ <| getLast_mem _
-
-@[simp] theorem getLast?_reverse (l : List α) : l.reverse.getLast? = l.head? := by cases l <;> simp
-
-@[simp] theorem head?_reverse (l : List α) : l.reverse.head? = l.getLast? := by
-  rw [← getLast?_reverse, reverse_reverse]
-
-/-! ### dropLast -/
-
-/-! NB: `dropLast` is the specification for `Array.pop`, so theorems about `List.dropLast`
-are often used for theorems about `Array.pop`.  -/
-
-theorem dropLast_cons_of_ne_nil {α : Type u} {x : α}
-    {l : List α} (h : l ≠ []) : (x :: l).dropLast = x :: l.dropLast := by
-  simp [dropLast, h]
-
-@[simp] theorem dropLast_append_of_ne_nil {α : Type u} {l : List α} :
-    ∀ (l' : List α) (_ : l ≠ []), (l' ++ l).dropLast = l' ++ l.dropLast
-  | [], _ => by simp only [nil_append]
-  | a :: l', h => by
-    rw [cons_append, dropLast, dropLast_append_of_ne_nil l' h, cons_append]
-    simp [h]
-
-theorem dropLast_append_cons : dropLast (l₁ ++ b::l₂) = l₁ ++ dropLast (b::l₂) := by
-  simp only [ne_eq, not_false_eq_true, dropLast_append_of_ne_nil]
-
-@[simp 1100] theorem dropLast_concat : dropLast (l₁ ++ [b]) = l₁ := by simp
-
-@[simp] theorem length_dropLast : ∀ (xs : List α), xs.dropLast.length = xs.length - 1
-  | [] => rfl
-  | x::xs => by simp
-
-@[simp] theorem getElem_dropLast : ∀ (xs : List α) (i : Nat) (h : i < xs.dropLast.length),
-    xs.dropLast[i] = xs[i]'(Nat.lt_of_lt_of_le h (length_dropLast .. ▸ Nat.pred_le _))
-  | _::_::_, 0, _ => rfl
-  | _::_::_, i+1, _ => getElem_dropLast _ i _
-
-@[deprecated getElem_dropLast (since := "2024-06-12")]
-theorem get_dropLast (xs : List α) (i : Fin xs.dropLast.length) :
-    xs.dropLast.get i = xs.get ⟨i, Nat.lt_of_lt_of_le i.isLt (length_dropLast .. ▸ Nat.pred_le _)⟩ := by
-  simp
-
-/-! ### nth element -/
-
-@[simp] theorem get_cons_cons_one : (a₁ :: a₂ :: as).get (1 : Fin (as.length + 2)) = a₂ := rfl
-
-theorem get!_cons_succ [Inhabited α] (l : List α) (a : α) (n : Nat) :
-    (a::l).get! (n+1) = get! l n := rfl
-
-theorem get!_cons_zero [Inhabited α] (l : List α) (a : α) : (a::l).get! 0 = a := rfl
-
-theorem get!_nil [Inhabited α] (n : Nat) : [].get! n = (default : α) := rfl
-
-theorem get!_len_le [Inhabited α] : ∀ {l : List α} {n}, length l ≤ n → l.get! n = (default : α)
-  | [], _, _ => rfl
-  | _ :: l, _+1, h => get!_len_le (l := l) <| Nat.le_of_succ_le_succ h
-
-theorem getElem?_of_mem {a} {l : List α} (h : a ∈ l) : ∃ n : Nat, l[n]? = some a :=
-  let ⟨n, _, e⟩ := getElem_of_mem h; ⟨n, e ▸ getElem?_eq_getElem _⟩
-
-theorem get?_of_mem {a} {l : List α} (h : a ∈ l) : ∃ n, l.get? n = some a :=
-  let ⟨⟨n, _⟩, e⟩ := get_of_mem h; ⟨n, e ▸ get?_eq_get _⟩
-
-theorem getElem?_mem {l : List α} {n : Nat} {a : α} (e : l[n]? = some a) : a ∈ l :=
-  let ⟨_, e⟩ := getElem?_eq_some.1 e; e ▸ getElem_mem ..
-
-theorem get?_mem {l : List α} {n a} (e : l.get? n = some a) : a ∈ l :=
-  let ⟨_, e⟩ := get?_eq_some.1 e; e ▸ get_mem ..
-
--- TODO(Mario): move somewhere else
-theorem Fin.exists_iff (p : Fin n → Prop) : (∃ i, p i) ↔ ∃ i h, p ⟨i, h⟩ :=
-  ⟨fun ⟨i, h⟩ => ⟨i.1, i.2, h⟩, fun ⟨i, hi, h⟩ => ⟨⟨i, hi⟩, h⟩⟩
-
-theorem mem_iff_getElem? {a} {l : List α} : a ∈ l ↔ ∃ n : Nat, l[n]? = some a := by
-  simp [getElem?_eq_some, mem_iff_getElem]
-
-theorem mem_iff_get? {a} {l : List α} : a ∈ l ↔ ∃ n, l.get? n = some a := by
-  simp [getElem?_eq_some, Fin.exists_iff, mem_iff_get]
-
-theorem get?_zero (l : List α) : l.get? 0 = l.head? := by cases l <;> rfl
-
-/--
-If one has `l[i]` in an expression and `h : l = l'`,
-`rw [h]` will give a "motive it not type correct" error, as it cannot rewrite the
-implicit `i < l.length` to `i < l'.length` directly. The theorem `getElem_of_eq` can be used to make
-such a rewrite, with `rw [getElem_of_eq h]`.
--/
-theorem getElem_of_eq {l l' : List α} (h : l = l') {i : Nat} (w : i < l.length) :
-    l[i] = l'[i]'(h ▸ w) := by cases h; rfl
-
-/--
-If one has `l.get i` in an expression (with `i : Fin l.length`) and `h : l = l'`,
-`rw [h]` will give a "motive it not type correct" error, as it cannot rewrite the
-`i : Fin l.length` to `Fin l'.length` directly. The theorem `get_of_eq` can be used to make
-such a rewrite, with `rw [get_of_eq h]`.
--/
-theorem get_of_eq {l l' : List α} (h : l = l') (i : Fin l.length) :
-    get l i = get l' ⟨i, h ▸ i.2⟩ := by cases h; rfl
-
-@[simp] theorem getElem_singleton (a : α) (h : i < 1) : [a][i] = a :=
-  match i, h with
-  | 0, _ => rfl
-
-@[deprecated getElem_singleton (since := "2024-06-12")]
-theorem get_singleton (a : α) (n : Fin 1) : get [a] n = a := by simp
-
-theorem getElem_zero {l : List α} (h : 0 < l.length) : l[0] = l.head (length_pos.mp h) :=
-  match l, h with
-  | _ :: _, _ => rfl
-
-theorem get_mk_zero : ∀ {l : List α} (h : 0 < l.length), l.get ⟨0, h⟩ = l.head (length_pos.mp h)
-  | _::_, _ => rfl
-
-theorem getElem_append_right' {l₁ l₂ : List α} {n : Nat} (h₁ : l₁.length ≤ n) (h₂) :
-    (l₁ ++ l₂)[n]'h₂ =
-      l₂[n - l₁.length]'(by rw [length_append] at h₂; exact Nat.sub_lt_left_of_lt_add h₁ h₂) :=
-  Option.some.inj <| by rw [← getElem?_eq_getElem, ← getElem?_eq_getElem, getElem?_append_right h₁]
-
-@[deprecated (since := "2024-06-12")]
-theorem get_append_right_aux {l₁ l₂ : List α} {n : Nat}
-  (h₁ : l₁.length ≤ n) (h₂ : n < (l₁ ++ l₂).length) : n - l₁.length < l₂.length := by
-  rw [length_append] at h₂
-  exact Nat.sub_lt_left_of_lt_add h₁ h₂
+/-! ### zipWithAll -/
+
+theorem getElem?_zipWithAll {f : Option α → Option β → γ} {i : Nat } :
+    (zipWithAll f as bs)[i]? = match as[i]?, bs[i]? with
+      | none, none => .none | a?, b? => some (f a? b?) := by
+  induction as generalizing bs i with
+  | nil => induction bs generalizing i with
+    | nil => simp
+    | cons b bs bih => cases i <;> simp_all
+  | cons a as aih => cases bs with
+    | nil =>
+      specialize @aih []
+      cases i <;> simp_all
+    | cons b bs => cases i <;> simp_all
+
+@[deprecated getElem?_zipWithAll (since := "2024-06-12")]
+theorem get?_zipWithAll {f : Option α → Option β → γ} :
+    (zipWithAll f as bs).get? i = match as.get? i, bs.get? i with
+      | none, none => .none | a?, b? => some (f a? b?) := by
+  simp [getElem?_zipWithAll]
 
 set_option linter.deprecated false in
-@[deprecated getElem_append_right' (since := "2024-06-12")]
-theorem get_append_right' {l₁ l₂ : List α} {n : Nat} (h₁ : l₁.length ≤ n) (h₂) :
-    (l₁ ++ l₂).get ⟨n, h₂⟩ = l₂.get ⟨n - l₁.length, get_append_right_aux h₁ h₂⟩ :=
-  Option.some.inj <| by rw [← get?_eq_get, ← get?_eq_get, get?_append_right h₁]
+@[deprecated getElem?_zipWithAll (since := "2024-06-07")] abbrev zipWithAll_get? := @get?_zipWithAll
 
-theorem getElem_of_append {l : List α} (eq : l = l₁ ++ a :: l₂) (h : l₁.length = n) :
-    l[n]'(eq ▸ h ▸ by simp_arith) = a := Option.some.inj <| by
-  rw [← getElem?_eq_getElem, eq, getElem?_append_right (h ▸ Nat.le_refl _), h]
-  simp
-
-@[deprecated (since := "2024-06-12")]
-theorem get_of_append_proof {l : List α}
-    (eq : l = l₁ ++ a :: l₂) (h : l₁.length = n) : n < length l := eq ▸ h ▸ by simp_arith
-
-set_option linter.deprecated false in
-@[deprecated getElem_of_append (since := "2024-06-12")]
-theorem get_of_append {l : List α} (eq : l = l₁ ++ a :: l₂) (h : l₁.length = n) :
-    l.get ⟨n, get_of_append_proof eq h⟩ = a := Option.some.inj <| by
-  rw [← get?_eq_get, eq, get?_append_right (h ▸ Nat.le_refl _), h, Nat.sub_self]; rfl
-
-@[simp] theorem getElem_replicate (a : α) {n : Nat} {m} (h : m < (replicate n a).length) :
-    (replicate n a)[m] = a :=
-  eq_of_mem_replicate (get_mem _ _ _)
-
-@[deprecated getElem_replicate (since := "2024-06-12")]
-theorem get_replicate (a : α) {n : Nat} (m : Fin _) : (replicate n a).get m = a := by
-  simp
-
-@[simp] theorem getLastD_concat (a b l) : @getLastD α (l ++ [b]) a = b := by
-  rw [getLastD_eq_getLast?, getLast?_concat]; rfl
-
-theorem getElem_cons_length (x : α) (xs : List α) (n : Nat) (h : n = xs.length) :
-    (x :: xs)[n]'(by simp [h]) = (x :: xs).getLast (cons_ne_nil x xs) := by
-  rw [getLast_eq_get]; cases h; rfl
-
-@[deprecated getElem_cons_length (since := "2024-06-12")]
-theorem get_cons_length (x : α) (xs : List α) (n : Nat) (h : n = xs.length) :
-    (x :: xs).get ⟨n, by simp [h]⟩ = (x :: xs).getLast (cons_ne_nil x xs) := by
-  simp [getElem_cons_length, h]
-
-theorem getElem!_of_getElem? [Inhabited α] : ∀ {l : List α} {n : Nat}, l[n]? = some a → l[n]! = a
-  | _a::_, 0, _ => by
-    rw [getElem!_pos] <;> simp_all
-  | _::l, _+1, e => by
-    simp at e
-    simp_all [getElem!_of_getElem? (l := l) e]
-
-theorem get!_of_get? [Inhabited α] : ∀ {l : List α} {n}, get? l n = some a → get! l n = a
-  | _a::_, 0, rfl => rfl
-  | _::l, _+1, e => get!_of_get? (l := l) e
-
-@[simp] theorem get!_eq_getD [Inhabited α] : ∀ (l : List α) n, l.get! n = l.getD n default
-  | [], _      => rfl
-  | _a::_, 0   => rfl
-  | _a::l, n+1 => get!_eq_getD l n
-
-/-! ### set -/
-
-@[simp] theorem set_eq_nil (l : List α) (n : Nat) (a : α) : l.set n a = [] ↔ l = [] := by
-  cases l <;> cases n <;> simp only [set]
-
-theorem set_comm (a b : α) : ∀ {n m : Nat} (l : List α), n ≠ m →
-    (l.set n a).set m b = (l.set m b).set n a
-  | _, _, [], _ => by simp
-  | n+1, 0, _ :: _, _ => by simp [set]
-  | 0, m+1, _ :: _, _ => by simp [set]
-  | n+1, m+1, x :: t, h =>
-    congrArg _ <| set_comm a b t fun h' => h <| Nat.succ_inj'.mpr h'
-
-@[simp]
-theorem set_set (a b : α) : ∀ (l : List α) (n : Nat), (l.set n a).set n b = l.set n b
-  | [], _ => by simp
-  | _ :: _, 0 => by simp [set]
-  | _ :: _, _+1 => by simp [set, set_set]
-
-theorem getElem_set (a : α) {m n} (l : List α) (h) :
-    (set l m a)[n]'h = if m = n then a else l[n]'(length_set .. ▸ h) := by
-  if h : m = n then
-    subst m; simp only [getElem_set_eq, ↓reduceIte]
-  else
-    simp [h]
-
-@[deprecated getElem_set (since := "2024-06-12")]
-theorem get_set (a : α) {m n} (l : List α) (h) :
-    (set l m a).get ⟨n, h⟩ = if m = n then a else l.get ⟨n, length_set .. ▸ h⟩ := by
-  simp [getElem_set]
-
-theorem mem_or_eq_of_mem_set : ∀ {l : List α} {n : Nat} {a b : α}, a ∈ l.set n b → a ∈ l ∨ a = b
-  | _ :: _, 0, _, _, h => ((mem_cons ..).1 h).symm.imp_left (.tail _)
-  | _ :: _, _+1, _, _, .head .. => .inl (.head ..)
-  | _ :: _, _+1, _, _, .tail _ h => (mem_or_eq_of_mem_set h).imp_left (.tail _)
-
-/-! ### all / any -/
-
-@[simp] theorem contains_nil [BEq α] : ([] : List α).contains a = false := rfl
-
-@[simp] theorem contains_cons [BEq α] :
-    (a :: as : List α).contains x = (a == x || as.contains x) := by
-  simp only [contains, elem]
-  split <;> simp_all
-
-theorem contains_eq_any_beq [BEq α] (l : List α) (a : α) : l.contains a = l.any (· == a) := by
-  induction l with simp | cons b l => cases b == a <;> simp [*]
-
-theorem not_all_eq_any_not (l : List α) (p : α → Bool) : (!l.all p) = l.any fun a => !p a := by
-  induction l with simp | cons _ _ ih => rw [ih]
-
-theorem not_any_eq_all_not (l : List α) (p : α → Bool) : (!l.any p) = l.all fun a => !p a := by
-  induction l with simp | cons _ _ ih => rw [ih]
-
-theorem or_all_distrib_left (l : List α) (p : α → Bool) (q : Bool) :
-    (q || l.all p) = l.all fun a => q || p a := by
-  induction l with simp | cons _ _ ih => rw [Bool.or_and_distrib_left, ih]
-
-theorem or_all_distrib_right (l : List α) (p : α → Bool) (q : Bool) :
-    (l.all p || q) = l.all fun a => p a || q := by
-  induction l with simp | cons _ _ ih => rw [Bool.or_and_distrib_right, ih]
-
-theorem and_any_distrib_left (l : List α) (p : α → Bool) (q : Bool) :
-    (q && l.any p) = l.any fun a => q && p a := by
-  induction l with simp | cons _ _ ih => rw [Bool.and_or_distrib_left, ih]
-
-theorem and_any_distrib_right (l : List α) (p : α → Bool) (q : Bool) :
-    (l.any p && q) = l.any fun a => p a && q := by
-  induction l with simp | cons _ _ ih => rw [Bool.and_or_distrib_right, ih]
-
-theorem any_eq_not_all_not (l : List α) (p : α → Bool) : l.any p = !l.all (!p .) := by
-  simp only [not_all_eq_any_not, Bool.not_not]
-
-theorem all_eq_not_any_not (l : List α) (p : α → Bool) : l.all p = !l.any (!p .) := by
-  simp only [not_any_eq_all_not, Bool.not_not]
-
-/-! ### reverse -/
-
-@[simp] theorem mem_reverseAux {x : α} : ∀ {as bs}, x ∈ reverseAux as bs ↔ x ∈ as ∨ x ∈ bs
-  | [], _ => ⟨.inr, fun | .inr h => h⟩
-  | a :: _, _ => by rw [reverseAux, mem_cons, or_assoc, or_left_comm, mem_reverseAux, mem_cons]
-
-@[simp] theorem mem_reverse {x : α} {as : List α} : x ∈ reverse as ↔ x ∈ as := by simp [reverse]
-
-/-! ### insert -/
-
-section insert
-variable [BEq α] [LawfulBEq α]
-
-@[simp] theorem insert_of_mem {l : List α} (h : a ∈ l) : l.insert a = l := by
-  simp [List.insert, h]
-
-@[simp] theorem insert_of_not_mem {l : List α} (h : a ∉ l) : l.insert a = a :: l := by
-  simp [List.insert, h]
-
-@[simp] theorem mem_insert_iff {l : List α} : a ∈ l.insert b ↔ a = b ∨ a ∈ l := by
-  if h : b ∈ l then
-    rw [insert_of_mem h]
-    constructor; {apply Or.inr}
-    intro
-    | Or.inl h' => rw [h']; exact h
-    | Or.inr h' => exact h'
-  else rw [insert_of_not_mem h, mem_cons]
-
-@[simp 1100] theorem mem_insert_self (a : α) (l : List α) : a ∈ l.insert a :=
-  mem_insert_iff.2 (Or.inl rfl)
-
-theorem mem_insert_of_mem {l : List α} (h : a ∈ l) : a ∈ l.insert b :=
-  mem_insert_iff.2 (Or.inr h)
-
-theorem eq_or_mem_of_mem_insert {l : List α} (h : a ∈ l.insert b) : a = b ∨ a ∈ l :=
-  mem_insert_iff.1 h
-
-@[simp] theorem length_insert_of_mem {l : List α} (h : a ∈ l) :
-    length (l.insert a) = length l := by rw [insert_of_mem h]
-
-@[simp] theorem length_insert_of_not_mem {l : List α} (h : a ∉ l) :
-    length (l.insert a) = length l + 1 := by rw [insert_of_not_mem h]; rfl
-
-end insert
-
-/-! ### erase -/
-
-section erase
-variable [BEq α]
-
-@[simp] theorem erase_nil (a : α) : [].erase a = [] := rfl
-
-theorem erase_cons (a b : α) (l : List α) :
-    (b :: l).erase a = if b == a then l else b :: l.erase a :=
-  if h : b == a then by simp [List.erase, h]
-  else by simp [List.erase, h, (beq_eq_false_iff_ne _ _).2 h]
-
-@[simp] theorem erase_cons_head [LawfulBEq α] (a : α) (l : List α) : (a :: l).erase a = l := by
-  simp [erase_cons]
-
-@[simp] theorem erase_cons_tail {a b : α} (l : List α) (h : ¬(b == a)) :
-    (b :: l).erase a = b :: l.erase a := by simp only [erase_cons, if_neg h]
-
-theorem erase_of_not_mem [LawfulBEq α] {a : α} : ∀ {l : List α}, a ∉ l → l.erase a = l
-  | [], _ => rfl
-  | b :: l, h => by
-    rw [mem_cons, not_or] at h
-    simp only [erase_cons, if_neg, erase_of_not_mem h.2, beq_iff_eq, Ne.symm h.1, not_false_eq_true]
-
-end erase
-
-/-! ### filter and partition -/
-
-@[simp] theorem filter_append {p : α → Bool} :
-    ∀ (l₁ l₂ : List α), filter p (l₁ ++ l₂) = filter p l₁ ++ filter p l₂
-  | [], l₂ => rfl
-  | a :: l₁, l₂ => by simp [filter]; split <;> simp [filter_append l₁]
-
-@[simp] theorem partition_eq_filter_filter (p : α → Bool) (l : List α) :
-    partition p l = (filter p l, filter (not ∘ p) l) := by simp [partition, aux] where
-  aux : ∀ l {as bs}, partition.loop p l (as, bs) =
-    (as.reverse ++ filter p l, bs.reverse ++ filter (not ∘ p) l)
-  | [] => by simp [partition.loop, filter]
-  | a :: l => by cases pa : p a <;> simp [partition.loop, pa, aux, filter, append_assoc]
-
-theorem filter_congr' {p q : α → Bool} :
-    ∀ {l : List α}, (∀ x ∈ l, p x ↔ q x) → filter p l = filter q l
-  | [], _ => rfl
-  | a :: l, h => by
-    rw [forall_mem_cons] at h; by_cases pa : p a
-    · simp [pa, h.1.1 pa, filter_congr' h.2]
-    · simp [pa, mt h.1.2 pa, filter_congr' h.2]
-
-/-! ### filterMap -/
-
-@[simp] theorem filterMap_nil (f : α → Option β) : filterMap f [] = [] := rfl
-
-@[simp] theorem filterMap_cons (f : α → Option β) (a : α) (l : List α) :
-    filterMap f (a :: l) =
-      match f a with
-      | none => filterMap f l
-      | some b => b :: filterMap f l := rfl
-
-theorem filterMap_cons_none {f : α → Option β} (a : α) (l : List α) (h : f a = none) :
-    filterMap f (a :: l) = filterMap f l := by simp only [filterMap, h]
-
-theorem filterMap_cons_some (f : α → Option β) (a : α) (l : List α) {b : β} (h : f a = some b) :
-    filterMap f (a :: l) = b :: filterMap f l := by simp only [filterMap, h]
-
-theorem filterMap_append {α β : Type _} (l l' : List α) (f : α → Option β) :
-    filterMap f (l ++ l') = filterMap f l ++ filterMap f l' := by
-  induction l <;> simp; split <;> simp [*]
-
-@[simp]
-theorem filterMap_eq_map (f : α → β) : filterMap (some ∘ f) = map f := by
-  funext l; induction l <;> simp [*]
-
-@[simp]
-theorem filterMap_eq_filter (p : α → Bool) :
-    filterMap (Option.guard (p ·)) = filter p := by
-  funext l
-  induction l with
-  | nil => rfl
-  | cons a l IH => by_cases pa : p a <;> simp [Option.guard, pa, ← IH]
-
-theorem filterMap_filterMap (f : α → Option β) (g : β → Option γ) (l : List α) :
-    filterMap g (filterMap f l) = filterMap (fun x => (f x).bind g) l := by
-  induction l with
-  | nil => rfl
-  | cons a l IH => cases h : f a <;> simp [*]
-
-theorem map_filterMap (f : α → Option β) (g : β → γ) (l : List α) :
-    map g (filterMap f l) = filterMap (fun x => (f x).map g) l := by
-  simp only [← filterMap_eq_map, filterMap_filterMap, Option.map_eq_bind]
-
-@[simp]
-theorem filterMap_map (f : α → β) (g : β → Option γ) (l : List α) :
-    filterMap g (map f l) = filterMap (g ∘ f) l := by
-  rw [← filterMap_eq_map, filterMap_filterMap]; rfl
-
-theorem filter_filterMap (f : α → Option β) (p : β → Bool) (l : List α) :
-    filter p (filterMap f l) = filterMap (fun x => (f x).filter p) l := by
-  rw [← filterMap_eq_filter, filterMap_filterMap]
-  congr; funext x; cases f x <;> simp [Option.filter, Option.guard]
-
-theorem filterMap_filter (p : α → Bool) (f : α → Option β) (l : List α) :
-    filterMap f (filter p l) = filterMap (fun x => if p x then f x else none) l := by
-  rw [← filterMap_eq_filter, filterMap_filterMap]
-  congr; funext x; by_cases h : p x <;> simp [Option.guard, h]
-
-@[simp] theorem filterMap_some (l : List α) : filterMap some l = l := by
-  erw [filterMap_eq_map, map_id]
-
-theorem map_filterMap_some_eq_filter_map_is_some (f : α → Option β) (l : List α) :
-    (l.filterMap f).map some = (l.map f).filter fun b => b.isSome := by
-  induction l <;> simp; split <;> simp [*]
-
-@[simp] theorem mem_filterMap (f : α → Option β) (l : List α) {b : β} :
-    b ∈ filterMap f l ↔ ∃ a, a ∈ l ∧ f a = some b := by
-  induction l <;> simp; split <;> simp [*, eq_comm]
-
-@[simp] theorem filterMap_join (f : α → Option β) (L : List (List α)) :
-    filterMap f (join L) = join (map (filterMap f) L) := by
-  induction L <;> simp [*, filterMap_append]
-
-theorem map_filterMap_of_inv (f : α → Option β) (g : β → α) (H : ∀ x : α, (f x).map g = some x)
-    (l : List α) : map g (filterMap f l) = l := by simp only [map_filterMap, H, filterMap_some]
-
-theorem map_filter (f : β → α) (l : List β) : filter p (map f l) = map f (filter (p ∘ f) l) := by
-  rw [← filterMap_eq_map, filter_filterMap, filterMap_filter]; rfl
-
-@[simp] theorem filter_filter (q) : ∀ l, filter p (filter q l) = filter (fun a => p a ∧ q a) l
-  | [] => rfl
-  | a :: l => by by_cases hp : p a <;> by_cases hq : q a <;> simp [hp, hq, filter_filter _ l]
-
-/-! ### find? -/
-
-theorem find?_cons_of_pos (l) (h : p a) : find? p (a :: l) = some a :=
-  by simp [find?, h]
-
-theorem find?_cons_of_neg (l) (h : ¬p a) : find? p (a :: l) = find? p l :=
-  by simp [find?, h]
-
-theorem find?_eq_none : find? p l = none ↔ ∀ x ∈ l, ¬ p x := by
-  induction l <;> simp [find?_cons]; split <;> simp [*]
-
-theorem find?_some : ∀ {l}, find? p l = some a → p a
-  | b :: l, H => by
-    by_cases h : p b <;> simp [find?, h] at H
-    · exact H ▸ h
-    · exact find?_some H
-
-@[simp] theorem mem_of_find?_eq_some : ∀ {l}, find? p l = some a → a ∈ l
-  | b :: l, H => by
-    by_cases h : p b <;> simp [find?, h] at H
-    · exact H ▸ .head _
-    · exact .tail _ (mem_of_find?_eq_some H)
-
-/-! ### findSome? -/
-
-theorem exists_of_findSome?_eq_some {l : List α} {f : α → Option β} (w : l.findSome? f = some b) :
-    ∃ a, a ∈ l ∧ f a = b := by
-  induction l with
-  | nil => simp_all
-  | cons h l ih =>
-    simp_all only [findSome?_cons, mem_cons, exists_eq_or_imp]
-    split at w <;> simp_all
-
-/-! ### takeWhile and dropWhile -/
-
-@[simp] theorem takeWhile_append_dropWhile (p : α → Bool) :
-    ∀ (l : List α), takeWhile p l ++ dropWhile p l = l
-  | [] => rfl
-  | x :: xs => by simp [takeWhile, dropWhile]; cases p x <;> simp [takeWhile_append_dropWhile p xs]
-
-theorem dropWhile_append {xs ys : List α} :
-    (xs ++ ys).dropWhile p =
-      if (xs.dropWhile p).isEmpty then ys.dropWhile p else xs.dropWhile p ++ ys := by
-  induction xs with
-  | nil => simp
-  | cons h t ih =>
-    simp only [cons_append, dropWhile_cons]
-    split <;> simp_all
-
-/-! ### enum, enumFrom -/
+/-! ### enumFrom -/
 
 @[simp] theorem enumFrom_length : ∀ {n} {l : List α}, (enumFrom n l).length = l.length
   | _, [] => rfl
   | _, _ :: _ => congrArg Nat.succ enumFrom_length
 
+/-! ### enum -/
+
 @[simp] theorem enum_length : (enum l).length = l.length :=
   enumFrom_length
+
+theorem enum_cons : (a::as).enum = (0, a) :: as.enumFrom 1 := rfl
+
+/-! ### minimum? -/
+
+@[simp] theorem minimum?_nil [Min α] : ([] : List α).minimum? = none := rfl
+
+-- We don't put `@[simp]` on `minimum?_cons`,
+-- because the definition in terms of `foldl` is not useful for proofs.
+theorem minimum?_cons [Min α] {xs : List α} : (x :: xs).minimum? = foldl min x xs := rfl
+
+@[simp] theorem minimum?_eq_none_iff {xs : List α} [Min α] : xs.minimum? = none ↔ xs = [] := by
+  cases xs <;> simp [minimum?]
+
+theorem minimum?_mem [Min α] (min_eq_or : ∀ a b : α, min a b = a ∨ min a b = b) :
+    {xs : List α} → xs.minimum? = some a → a ∈ xs := by
+  intro xs
+  match xs with
+  | nil => simp
+  | x :: xs =>
+    simp only [minimum?_cons, Option.some.injEq, List.mem_cons]
+    intro eq
+    induction xs generalizing x with
+    | nil =>
+      simp at eq
+      simp [eq]
+    | cons y xs ind =>
+      simp at eq
+      have p := ind _ eq
+      cases p with
+      | inl p =>
+        cases min_eq_or x y with | _ q => simp [p, q]
+      | inr p => simp [p, mem_cons]
+
+theorem le_minimum?_iff [Min α] [LE α]
+    (le_min_iff : ∀ a b c : α, a ≤ min b c ↔ a ≤ b ∧ a ≤ c) :
+    {xs : List α} → xs.minimum? = some a → ∀ x, x ≤ a ↔ ∀ b, b ∈ xs → x ≤ b
+  | nil => by simp
+  | cons x xs => by
+    rw [minimum?]
+    intro eq y
+    simp only [Option.some.injEq] at eq
+    induction xs generalizing x with
+    | nil =>
+      simp at eq
+      simp [eq]
+    | cons z xs ih =>
+      simp at eq
+      simp [ih _ eq, le_min_iff, and_assoc]
+
+-- This could be refactored by designing appropriate typeclasses to replace `le_refl`, `min_eq_or`,
+-- and `le_min_iff`.
+theorem minimum?_eq_some_iff [Min α] [LE α] [anti : Antisymm ((· : α) ≤ ·)]
+    (le_refl : ∀ a : α, a ≤ a)
+    (min_eq_or : ∀ a b : α, min a b = a ∨ min a b = b)
+    (le_min_iff : ∀ a b c : α, a ≤ min b c ↔ a ≤ b ∧ a ≤ c) {xs : List α} :
+    xs.minimum? = some a ↔ a ∈ xs ∧ ∀ b, b ∈ xs → a ≤ b := by
+  refine ⟨fun h => ⟨minimum?_mem min_eq_or h, (le_minimum?_iff le_min_iff h _).1 (le_refl _)⟩, ?_⟩
+  intro ⟨h₁, h₂⟩
+  cases xs with
+  | nil => simp at h₁
+  | cons x xs =>
+    exact congrArg some <| anti.1
+      ((le_minimum?_iff le_min_iff (xs := x::xs) rfl _).1 (le_refl _) _ h₁)
+      (h₂ _ (minimum?_mem min_eq_or (xs := x::xs) rfl))
 
 /-! ### maximum? -/
 
 @[simp] theorem maximum?_nil [Max α] : ([] : List α).maximum? = none := rfl
 
--- We don't put `@[simp]` on `minimum?_cons`,
+-- We don't put `@[simp]` on `maximum?_cons`,
 -- because the definition in terms of `foldl` is not useful for proofs.
 theorem maximum?_cons [Max α] {xs : List α} : (x :: xs).maximum? = foldl max x xs := rfl
 
@@ -1860,48 +1811,41 @@ theorem maximum?_eq_some_iff [Max α] [LE α] [anti : Antisymm ((· : α) ≤ ·
       (h₂ _ (maximum?_mem max_eq_or (xs := x::xs) rfl))
       ((maximum?_le_iff max_le_iff (xs := x::xs) rfl _).1 (le_refl _) _ h₁)
 
-/-! ### lt -/
+/-! ### mapM -/
 
-theorem lt_irrefl' [LT α] (lt_irrefl : ∀ x : α, ¬x < x) (l : List α) : ¬l < l := by
-  induction l with
-  | nil => nofun
-  | cons a l ih => intro
-    | .head _ _ h => exact lt_irrefl _ h
-    | .tail _ _ h => exact ih h
+/-- Alternate (non-tail-recursive) form of mapM for proofs. -/
+def mapM' [Monad m] (f : α → m β) : List α → m (List β)
+  | [] => pure []
+  | a :: l => return (← f a) :: (← l.mapM' f)
 
-theorem lt_trans' [LT α] [DecidableRel (@LT.lt α _)]
-    (lt_trans : ∀ {x y z : α}, x < y → y < z → x < z)
-    (le_trans : ∀ {x y z : α}, ¬x < y → ¬y < z → ¬x < z)
-    {l₁ l₂ l₃ : List α} (h₁ : l₁ < l₂) (h₂ : l₂ < l₃) : l₁ < l₃ := by
-  induction h₁ generalizing l₃ with
-  | nil => let _::_ := l₃; exact List.lt.nil ..
-  | @head a l₁ b l₂ ab =>
-    match h₂ with
-    | .head l₂ l₃ bc => exact List.lt.head _ _ (lt_trans ab bc)
-    | .tail _ cb ih =>
-      exact List.lt.head _ _ <| Decidable.by_contra (le_trans · cb ab)
-  | @tail a l₁ b l₂ ab ba h₁ ih2 =>
-    match h₂ with
-    | .head l₂ l₃ bc =>
-      exact List.lt.head _ _ <| Decidable.by_contra (le_trans ba · bc)
-    | .tail bc cb ih =>
-      exact List.lt.tail (le_trans ab bc) (le_trans cb ba) (ih2 ih)
+@[simp] theorem mapM'_nil [Monad m] {f : α → m β} : mapM' f [] = pure [] := rfl
+@[simp] theorem mapM'_cons [Monad m] {f : α → m β} :
+    mapM' f (a :: l) = return ((← f a) :: (← l.mapM' f)) :=
+  rfl
 
-theorem lt_antisymm' [LT α]
-    (lt_antisymm : ∀ {x y : α}, ¬x < y → ¬y < x → x = y)
-    {l₁ l₂ : List α} (h₁ : ¬l₁ < l₂) (h₂ : ¬l₂ < l₁) : l₁ = l₂ := by
-  induction l₁ generalizing l₂ with
-  | nil =>
-    cases l₂ with
-    | nil => rfl
-    | cons b l₂ => cases h₁ (.nil ..)
-  | cons a l₁ ih =>
-    cases l₂ with
-    | nil => cases h₂ (.nil ..)
-    | cons b l₂ =>
-      have ab : ¬a < b := fun ab => h₁ (.head _ _ ab)
-      cases lt_antisymm ab (fun ba => h₂ (.head _ _ ba))
-      rw [ih (fun ll => h₁ (.tail ab ab ll)) (fun ll => h₂ (.tail ab ab ll))]
+theorem mapM'_eq_mapM [Monad m] [LawfulMonad m] (f : α → m β) (l : List α) :
+    mapM' f l = mapM f l := by simp [go, mapM] where
+  go : ∀ l acc, mapM.loop f l acc = return acc.reverse ++ (← mapM' f l)
+    | [], acc => by simp [mapM.loop, mapM']
+    | a::l, acc => by simp [go l, mapM.loop, mapM']
 
+@[simp] theorem mapM_nil [Monad m] (f : α → m β) : [].mapM f = pure [] := rfl
+
+@[simp] theorem mapM_cons [Monad m] [LawfulMonad m] (f : α → m β) :
+    (a :: l).mapM f = (return (← f a) :: (← l.mapM f)) := by simp [← mapM'_eq_mapM, mapM']
+
+@[simp] theorem mapM_append [Monad m] [LawfulMonad m] (f : α → m β) {l₁ l₂ : List α} :
+    (l₁ ++ l₂).mapM f = (return (← l₁.mapM f) ++ (← l₂.mapM f)) := by induction l₁ <;> simp [*]
+
+/-! ### forM -/
+
+-- We use `List.forM` as the simp normal form, rather that `ForM.forM`.
+-- As such we need to replace `List.forM_nil` and `List.forM_cons`:
+
+@[simp] theorem forM_nil' [Monad m] : ([] : List α).forM f = (pure .unit : m PUnit) := rfl
+
+@[simp] theorem forM_cons' [Monad m] :
+    (a::as).forM f = (f a >>= fun _ => as.forM f : m PUnit) :=
+  List.forM_cons _ _ _
 
 end List
