src/Init/Data/Fin/Basic.lean
@@ -210,4 +210,7 @@ theorem val_add_one_le_of_lt {n : Nat} {a b : Fin n} (h : a < b) : (a : Nat) + 1
 
 theorem val_add_one_le_of_gt {n : Nat} {a b : Fin n} (h : a > b) : (b : Nat) + 1 ≤ (a : Nat) := h
 
+theorem exists_iff {p : Fin n → Prop} : (Exists fun i => p i) ↔ Exists fun i => Exists fun h => p ⟨i, h⟩ :=
+  ⟨fun ⟨⟨i, hi⟩, hpi⟩ => ⟨i, hi, hpi⟩, fun ⟨i, hi, hpi⟩ => ⟨⟨i, hi⟩, hpi⟩⟩
+
 end Fin
