src/Init/Data/List/Notation.lean
@@ -1,0 +1,53 @@
+/-
+Copyright (c) 2016 Microsoft Corporation. All rights reserved.
+Released under Apache 2.0 license as described in the file LICENSE.
+Author: Leonardo de Moura
+-/
+prelude
+import Init.Data.Nat.Div
+
+/-!
+# Notation for `List` literals.
+-/
+
+set_option linter.missingDocs true -- keep it documented
+open Decidable List
+
+/--
+The syntax `[a, b, c]` is shorthand for `a :: b :: c :: []`, or
+`List.cons a (List.cons b (List.cons c List.nil))`. It allows conveniently constructing
+list literals.
+
+For lists of length at least 64, an alternative desugaring strategy is used
+which uses let bindings as intermediates as in
+`let left := [d, e, f]; a :: b :: c :: left` to avoid creating very deep expressions.
+Note that this changes the order of evaluation, although it should not be observable
+unless you use side effecting operations like `dbg_trace`.
+-/
+syntax "[" withoutPosition(term,*,?) "]"  : term
+
+/--
+Auxiliary syntax for implementing `[$elem,*]` list literal syntax.
+The syntax `%[a,b,c|tail]` constructs a value equivalent to `a::b::c::tail`.
+It uses binary partitioning to construct a tree of intermediate let bindings as in
+`let left := [d, e, f]; a :: b :: c :: left` to avoid creating very deep expressions.
+-/
+syntax "%[" withoutPosition(term,*,? " | " term) "]" : term
+
+namespace Lean
+
+macro_rules
+  | `([ $elems,* ]) => do
+    -- NOTE: we do not have `TSepArray.getElems` yet at this point
+    let rec expandListLit (i : Nat) (skip : Bool) (result : TSyntax `term) : MacroM Syntax := do
+      match i, skip with
+      | 0,   _     => pure result
+      | i+1, true  => expandListLit i false result
+      | i+1, false => expandListLit i true  (← ``(List.cons $(⟨elems.elemsAndSeps.get! i⟩) $result))
+    let size := elems.elemsAndSeps.size
+    if size < 64 then
+      expandListLit size (size % 2 == 0) (← ``(List.nil))
+    else
+      `(%[ $elems,* | List.nil ])
+
+end Lean
